Wrapping up (SLD + extraction + cosmetics)

extracted/interpreter.hs
@@ -1,0 +1,389 @@
+module Interpreter where
+
+import qualified Prelude
+
+__ :: any
+__ = Prelude.error "Logical or arity value used"
+
+eq_rect :: a1 -> a2 -> a1 -> a2
+eq_rect _ f _ =
+  f
+
+eq_rec :: a1 -> a2 -> a1 -> a2
+eq_rec =
+  eq_rect
+
+eq_rec_r :: a1 -> a2 -> a1 -> a2
+eq_rec_r =
+  eq_rec
+
+data Bool =
+   True
+ | False
+
+orb :: Bool -> Bool -> Bool
+orb b1 b2 =
+  case b1 of {
+   True -> True;
+   False -> b2}
+
+data Nat =
+   O
+ | S Nat
+
+nat_rect :: a1 -> (Nat -> a1 -> a1) -> Nat -> a1
+nat_rect f f0 n =
+  case n of {
+   O -> f;
+   S n0 -> f0 n0 (nat_rect f f0 n0)}
+
+nat_rec :: a1 -> (Nat -> a1 -> a1) -> Nat -> a1
+nat_rec =
+  nat_rect
+
+data Option a =
+   Some a
+ | None
+
+data Prod a b =
+   Pair a b
+
+fst :: (Prod a1 a2) -> a1
+fst p0 =
+  case p0 of {
+   Pair x _ -> x}
+
+snd :: (Prod a1 a2) -> a2
+snd p0 =
+  case p0 of {
+   Pair _ y -> y}
+
+data List a =
+   Nil
+ | Cons a (List a)
+
+app :: (List a1) -> (List a1) -> List a1
+app l m =
+  case l of {
+   Nil -> m;
+   Cons a l1 -> Cons a (app l1 m)}
+
+type Sig a = a
+  -- singleton inductive, whose constructor was exist
+  
+data SigT a p =
+   ExistT a p
+
+proj1_sig :: a1 -> a1
+proj1_sig e =
+  e
+
+data Sumbool =
+   Left
+ | Right
+
+acc_rect :: (a1 -> () -> (a1 -> () -> a2) -> a2) -> a1 -> a2
+acc_rect f x =
+  f x __ (\y _ -> acc_rect f y)
+
+well_founded_induction_type :: (a1 -> (a1 -> () -> a2) -> a2) -> a1 -> a2
+well_founded_induction_type x a =
+  acc_rect (\x0 _ x1 -> x x0 x1) a
+
+well_founded_induction :: (a1 -> (a1 -> () -> a2) -> a2) -> a1 -> a2
+well_founded_induction =
+  well_founded_induction_type
+
+eqb :: Nat -> Nat -> Bool
+eqb n m =
+  case n of {
+   O -> case m of {
+         O -> True;
+         S _ -> False};
+   S n' -> case m of {
+            O -> False;
+            S m' -> eqb n' m'}}
+
+eq_dec :: Nat -> Nat -> Sumbool
+eq_dec n =
+  nat_rec (\m -> case m of {
+                  O -> Left;
+                  S _ -> Right}) (\_ iHn m ->
+    case m of {
+     O -> Right;
+     S m0 -> iHn m0}) n
+
+map :: (a1 -> a2) -> (List a1) -> List a2
+map f l =
+  case l of {
+   Nil -> Nil;
+   Cons a t -> Cons (f a) (map f t)}
+
+type Name = Nat
+
+data Term =
+   Var Name
+ | Cst Name
+ | Con Name Term Term
+
+occurs :: Name -> Term -> Bool
+occurs n t =
+  case t of {
+   Var x -> eqb n x;
+   Cst _ -> False;
+   Con _ l r -> orb (occurs n l) (occurs n r)}
+
+type Subst = List (Prod Name Term)
+
+empty_subst :: Subst
+empty_subst =
+  Nil
+
+singleton_subst :: Name -> Term -> List (Prod Name Term)
+singleton_subst n t =
+  Cons (Pair n t) Nil
+
+image :: Subst -> Name -> Option Term
+image s n =
+  case s of {
+   Nil -> None;
+   Cons p0 tl ->
+    case p0 of {
+     Pair m t -> case eq_dec m n of {
+                  Left -> Some t;
+                  Right -> image tl n}}}
+
+apply_subst :: Subst -> Term -> Term
+apply_subst s t =
+  case t of {
+   Var n -> case image s n of {
+             Some t' -> t';
+             None -> t};
+   Cst _ -> t;
+   Con n l r -> Con n (apply_subst s l) (apply_subst s r)}
+
+compose :: Subst -> Subst -> Subst
+compose s1 s2 =
+  app (map (\p0 -> Pair (fst p0) (apply_subst s2 (snd p0))) s1) s2
+
+data Unification_step_outcome =
+   NonUnifiable
+ | Same
+ | VarSubst Name Term
+
+create :: Name -> Term -> Unification_step_outcome
+create n t =
+  case occurs n t of {
+   True -> NonUnifiable;
+   False -> VarSubst n t}
+
+unification_step :: Term -> Term -> Unification_step_outcome
+unification_step t1 t2 =
+  case t1 of {
+   Var n1 ->
+    case t2 of {
+     Var n2 -> case eq_dec n1 n2 of {
+                Left -> Same;
+                Right -> create n1 t2};
+     _ -> create n1 t2};
+   Cst n1 ->
+    case t2 of {
+     Var n2 -> create n2 t1;
+     Cst n2 -> case eq_dec n1 n2 of {
+                Left -> Same;
+                Right -> NonUnifiable};
+     Con _ _ _ -> NonUnifiable};
+   Con n1 l1 r1 ->
+    case t2 of {
+     Var n2 -> create n2 t1;
+     Cst _ -> NonUnifiable;
+     Con n2 l2 r2 ->
+      case eq_dec n1 n2 of {
+       Left ->
+        case unification_step l1 l2 of {
+         Same -> unification_step r1 r2;
+         x -> x};
+       Right -> NonUnifiable}}}
+
+data Mgu =
+   MguNonUnifiable Term Term
+ | MguSame Term Term
+ | MguVarSubstNone Term Term Name Term Mgu
+ | MguVarSubstSome Term Term Name Term Subst Subst Mgu
+
+mgu_exists :: Term -> Term -> SigT (Option Subst) Mgu
+mgu_exists t1 t2 =
+  let {
+   h = well_founded_induction (\x h ->
+         eq_rec_r __ (\h0 ->
+           case x of {
+            Pair t3 t4 ->
+             let {u = unification_step t3 t4} in
+             case u of {
+              NonUnifiable -> ExistT None (MguNonUnifiable t3 t4);
+              Same -> ExistT (Some empty_subst) (MguSame t3 t4);
+              VarSubst n t ->
+               let {
+                h1 = h0 (Pair (apply_subst (singleton_subst n t) t3)
+                       (apply_subst (singleton_subst n t) t4))}
+               in
+               let {h2 = h1 __} in
+               case h2 of {
+                ExistT x0 m ->
+                 case x0 of {
+                  Some s -> ExistT (Some (compose (singleton_subst n t) s))
+                   (MguVarSubstSome t3 t4 n t s
+                   (compose (singleton_subst n t) s) m);
+                  None -> ExistT None (MguVarSubstNone t3 t4 n t m)}}}}) __ h)
+         (Pair t1 t2)}
+  in
+  eq_rec_r __ (\h0 -> h0) __ h
+
+data Goal =
+   Fail
+ | Cut
+ | Unify Term Term
+ | Disj Goal Goal
+ | Conj Goal Goal
+ | Fresh (Name -> Goal)
+ | Invoke Name Term
+
+type Rel = Term -> Goal
+
+type Def = Rel
+
+type Spec = Name -> Def
+
+p :: Spec
+p =
+  Prelude.error "AXIOM TO BE REALIZED"
+
+data Stream a =
+   Nil0
+ | Cons0 a (Stream a)
+
+helper :: (Stream a1) -> Stream a1
+helper s =
+  s
+
+data State' =
+   Leaf Goal Subst Nat
+ | Sum State' State'
+ | Prod0 State' Goal
+
+state'_rect :: (Goal -> Subst -> Nat -> a1) -> (State' -> a1 -> State' -> a1
+               -> a1) -> (State' -> a1 -> Goal -> a1) -> State' -> a1
+state'_rect f f0 f1 s =
+  case s of {
+   Leaf g s0 n -> f g s0 n;
+   Sum s0 s1 -> f0 s0 (state'_rect f f0 f1 s0) s1 (state'_rect f f0 f1 s1);
+   Prod0 s0 g -> f1 s0 (state'_rect f f0 f1 s0) g}
+
+state'_rec :: (Goal -> Subst -> Nat -> a1) -> (State' -> a1 -> State' -> a1
+              -> a1) -> (State' -> a1 -> Goal -> a1) -> State' -> a1
+state'_rec =
+  state'_rect
+
+data State0 =
+   Stop
+ | State State'
+
+data Label =
+   Step
+ | Answer Subst Nat
+
+data Eval_step =
+   EsFail Subst Nat
+ | EsCut Subst Nat
+ | EsUnifyFail Term Term Subst Nat Mgu
+ | EsUnifySuccess Term Term Subst Subst Nat Mgu
+ | EsDisj Goal Goal Subst Nat
+ | EsConj Goal Goal Subst Nat
+ | EsFresh (Name -> Goal) Subst Nat
+ | EsInvoke Name Term Subst Nat
+ | EsSumE State' State' Label Eval_step
+ | EsSumNE State' State' State' Label Eval_step
+ | EsProdSE State' Goal Eval_step
+ | EsProdAE State' Goal Subst Nat Eval_step
+ | EsProdSNE State' Goal State' Eval_step
+ | EsProdANE State' Goal Subst Nat State' Eval_step
+
+eval_step_exists :: State' -> SigT Label (SigT State0 Eval_step)
+eval_step_exists st' =
+  state'_rec (\g s n ->
+    case g of {
+     Fail -> ExistT Step (ExistT Stop (EsFail s n));
+     Cut -> ExistT (Answer s n) (ExistT Stop (EsCut s n));
+     Unify t t0 ->
+      let {h = mgu_exists (apply_subst s t) (apply_subst s t0)} in
+      case h of {
+       ExistT x m ->
+        case x of {
+         Some s0 -> ExistT (Answer (compose s s0) n) (ExistT Stop
+          (EsUnifySuccess t t0 s s0 n m));
+         None -> ExistT Step (ExistT Stop (EsUnifyFail t t0 s n m))}};
+     Disj g1 g2 -> ExistT Step (ExistT (State (Sum (Leaf g1 s n) (Leaf g2 s
+      n))) (EsDisj g1 g2 s n));
+     Conj g1 g2 -> ExistT Step (ExistT (State (Prod0 (Leaf g1 s n) g2))
+      (EsConj g1 g2 s n));
+     Fresh g0 -> ExistT Step (ExistT (State (Leaf (g0 n) s (S n))) (EsFresh
+      g0 s n));
+     Invoke n0 t -> ExistT Step (ExistT (State (Leaf (proj1_sig (p n0) t) s
+      n)) (EsInvoke n0 t s n))}) (\st'1 iHst'1 st'2 _ ->
+    case iHst'1 of {
+     ExistT l1 s ->
+      case s of {
+       ExistT st1 iH1 ->
+        case st1 of {
+         Stop -> ExistT l1 (ExistT (State st'2) (EsSumE st'1 st'2 l1 iH1));
+         State s0 -> ExistT l1 (ExistT (State (Sum st'2 s0)) (EsSumNE st'1 s0
+          st'2 l1 iH1))}}}) (\st'0 iHst' g ->
+    case iHst' of {
+     ExistT l s ->
+      case s of {
+       ExistT st iH ->
+        case st of {
+         Stop ->
+          case l of {
+           Step -> ExistT Step (ExistT Stop (EsProdSE st'0 g iH));
+           Answer s0 n -> ExistT Step (ExistT (State (Leaf g s0 n)) (EsProdAE
+            st'0 g s0 n iH))};
+         State s0 ->
+          case l of {
+           Step -> ExistT Step (ExistT (State (Prod0 s0 g)) (EsProdSNE st'0 g
+            s0 iH));
+           Answer s1 n -> ExistT Step (ExistT (State (Sum (Leaf g s1 n)
+            (Prod0 s0 g))) (EsProdANE st'0 g s1 n s0 iH))}}}}) st'
+
+type Trace = Stream Label
+
+data Op_sem =
+   OsStop
+ | OsState State' Label State0 Trace Eval_step Op_sem
+
+trace_from :: State0 -> Trace
+trace_from st =
+  case st of {
+   Stop -> Nil0;
+   State st' ->
+    case eval_step_exists st' of {
+     ExistT l s -> case s of {
+                    ExistT st'' _ -> Cons0 l (trace_from st'')}}}
+
+trace_from_correct :: State0 -> Op_sem
+trace_from_correct st =
+  case st of {
+   Stop -> eq_rec_r (helper (trace_from Stop)) OsStop (trace_from Stop);
+   State s ->
+    eq_rec_r (helper (trace_from (State s)))
+      (let {s0 = eval_step_exists s} in
+       case s0 of {
+        ExistT x s1 ->
+         case s1 of {
+          ExistT x0 e -> OsState s x x0 (trace_from x0) e
+           (trace_from_correct x0)}}) (trace_from (State s))}
+
+op_sem_exists :: State0 -> SigT Trace Op_sem
+op_sem_exists st =
+  ExistT (trace_from st) (trace_from_correct st)
+
