src/DenotationalSem.v
@@ -1,3 +1,5 @@
+Add LoadPath "~/JB/minikanren-coq/src/".
+
 Require Import List.
 Require Import Coq.Lists.ListSet.
 Import ListNotations.
@@ -27,8 +29,11 @@ refine (
 simpl. rewrite lg. rewrite rg. reflexivity.
 Defined.
 
-Lemma gt_fun_eq_apply (f1 f2 : gt_fun) (t : term) (feq : gt_fun_eq f1 f2) :
-  gt_eq (apply_gt_fun f1 t) (apply_gt_fun f2 t).
+Lemma gt_fun_eq_apply
+      (f1 f2 : gt_fun)
+      (t : term)
+      (FEQ : gt_fun_eq f1 f2) :
+      gt_eq (apply_gt_fun f1 t) (apply_gt_fun f2 t).
 Proof.
   induction t.
   { simpl. auto. }
@@ -45,11 +50,11 @@ Qed.
 Lemma apply_gt_fun_fv
       (f1 f2 : gt_fun)
       (t : term)
-      (f_fv_eq : forall x, (In x (fv_term t)) -> gt_eq (f1 x) (f2 x)) :
+      (F12_FV_EQ : forall x, (In x (fv_term t)) -> gt_eq (f1 x) (f2 x)) :
       gt_eq (apply_gt_fun f1 t) (apply_gt_fun f2 t).
 Proof.
   induction t.
-  { simpl. apply f_fv_eq. simpl. auto. }
+  { simpl. apply F12_FV_EQ. simpl. auto. }
   { unfold gt_eq. auto. }
   { unfold gt_eq. simpl.
     remember (apply_gt_fun f1 t1) as p11. destruct p11.
@@ -58,35 +63,35 @@ Proof.
     remember (apply_gt_fun f2 t2) as p22. destruct p22.
     simpl.
     assert (x = x1).
-    { apply IHt1. intros. apply f_fv_eq. unfold fv_term.
+    { apply IHt1. intros. apply F12_FV_EQ. unfold fv_term.
       apply (set_union_intro name_eq_dec). left. auto. }
     assert (x0 = x2).
-    { apply IHt2. intros. apply f_fv_eq. unfold fv_term.
+    { apply IHt2. intros. apply F12_FV_EQ. unfold fv_term.
       apply (set_union_intro name_eq_dec). right. auto. }
     subst. auto. }
 Qed.
 
 Lemma gt_fun_eq_trans
       (f1 f2 f3 : gt_fun)
-      (eq12 : gt_fun_eq f1 f2)
-      (eq23 : gt_fun_eq f2 f3) :
+      (EQ12 : gt_fun_eq f1 f2)
+      (EQ23 : gt_fun_eq f2 f3) :
       gt_fun_eq f1 f3.
 Proof.
-  revert eq12 eq23. unfold gt_fun_eq. unfold gt_eq. intros.
-  rewrite eq12. auto.
+  revert EQ12 EQ23. unfold gt_fun_eq. unfold gt_eq. intros.
+  rewrite EQ12. auto.
 Qed.
 
 Lemma subst_of_gt
       (t : term)
       (s : subst)
       (f : gt_fun)
-      (H : forall x : name, In x (fv_term t) -> image s x = Some (proj1_sig (f x))) :
+      (FV_IMG : forall x : name, In x (fv_term t) -> image s x = Some (proj1_sig (f x))) :
       apply_subst s t = proj1_sig (apply_gt_fun f t).
 Proof.
   induction t.
   { simpl. replace (image s n) with (Some (proj1_sig (f n))).
     { auto. }
-    { symmetry. apply H. constructor. auto. } }
+    { symmetry. apply FV_IMG. constructor. auto. } }
   { auto. }
   { simpl.
     destruct (apply_gt_fun f t1).
@@ -95,17 +100,20 @@ Proof.
     replace x with (apply_subst s t1).
     { replace x0 with (apply_subst s t2).
       { auto. }
-      { apply IHt2. intros. apply H.
+      { apply IHt2. intros. apply FV_IMG.
         apply set_union_intro2. auto. } }
-    { apply IHt1. intros. apply H.
+    { apply IHt1. intros. apply FV_IMG.
       apply set_union_intro1. auto. } }
 Qed.
 
 Definition subst_gt_fun_compose (s : subst) (f : gt_fun) : gt_fun :=
   fun x => apply_gt_fun f (apply_subst s (Var x)).
 
-Lemma gt_fun_apply_compose (s : subst) (f : gt_fun) (t : term) :
-  gt_eq (apply_gt_fun (subst_gt_fun_compose s f) t) (apply_gt_fun f (apply_subst s t)).
+Lemma gt_fun_apply_compose
+      (s : subst)
+      (f : gt_fun)
+      (t : term) :
+      gt_eq (apply_gt_fun (subst_gt_fun_compose s f) t) (apply_gt_fun f (apply_subst s t)).
 Proof.
   induction t.
   { reflexivity. }
@@ -123,11 +131,11 @@ Qed.
 
 Lemma gt_fun_eq_compose
       (f1 f2 : gt_fun)
-      (eq : gt_fun_eq f1 f2)
+      (EQ : gt_fun_eq f1 f2)
       (s : subst) :
       gt_fun_eq (subst_gt_fun_compose s f1) (subst_gt_fun_compose s f2).
 Proof.
-  unfold gt_fun_eq. unfold gt_fun_eq in eq. unfold subst_gt_fun_compose.
+  unfold gt_fun_eq. unfold gt_fun_eq in EQ. unfold subst_gt_fun_compose.
   intro. induction (apply_subst s (Var x)).
   { simpl. auto. }
   { reflexivity. }
@@ -145,11 +153,11 @@ Qed.
 Lemma gt_fun_compose_eq
       (f : gt_fun)
       (s1 s2 : subst)
-      (eq : forall t, apply_subst s1 t = apply_subst s2 t) :
+      (EQ : forall t, apply_subst s1 t = apply_subst s2 t) :
       gt_fun_eq (subst_gt_fun_compose s1 f) (subst_gt_fun_compose s2 f).
 Proof.
   unfold gt_fun_eq. unfold subst_gt_fun_compose. unfold gt_eq.
-  intro. rewrite eq. auto.
+  intro. rewrite EQ. auto.
 Qed.
 
 Lemma subst_gt_fun_compose_assoc_subst
@@ -168,165 +176,168 @@ Proof.
 Qed.
 
 Inductive in_denotational_sem_goal : goal -> gt_fun -> Prop :=
-| dsgUnify  : forall f t1 t2 (UnH : gt_eq (apply_gt_fun f t1) (apply_gt_fun f t2)),
+| dsgCut    : forall f, in_denotational_sem_goal Cut f
+| dsgUnify  : forall f t1 t2 (UNI : gt_eq (apply_gt_fun f t1) (apply_gt_fun f t2)),
                              in_denotational_sem_goal (Unify t1 t2) f
-| dsgDisjL  : forall f g1 g2 (Hg : in_denotational_sem_goal g1 f),
+| dsgDisjL  : forall f g1 g2 (DSG : in_denotational_sem_goal g1 f),
                              in_denotational_sem_goal (Disj g1 g2) f
-| dsgDisjR  : forall f g1 g2 (Hg : in_denotational_sem_goal g2 f),
+| dsgDisjR  : forall f g1 g2 (DSG : in_denotational_sem_goal g2 f),
                              in_denotational_sem_goal (Disj g1 g2) f
-| dsgConj   : forall f g1 g2 (Hg1 : in_denotational_sem_goal g1 f)
-                             (Hg2 : in_denotational_sem_goal g2 f),
+| dsgConj   : forall f g1 g2 (DSG_L : in_denotational_sem_goal g1 f)
+                             (DSG_R : in_denotational_sem_goal g2 f),
                              in_denotational_sem_goal (Conj g1 g2) f
-| dsgFresh  : forall f fn a fg (fvH : ~ is_fv_of_goal a (Fresh fg))
-                               (Hg : in_denotational_sem_goal (fg a) fn)
-                               (Hease : forall (x : name) (neq : x <> a), gt_eq (fn x) (f x)),
+| dsgFresh  : forall f fn a fg (A_NOT_FV : ~ is_fv_of_goal a (Fresh fg))
+                               (DSG : in_denotational_sem_goal (fg a) fn)
+                               (EASE : forall (x : name) (neq : x <> a), gt_eq (fn x) (f x)),
                                in_denotational_sem_goal (Fresh fg) f
-| dsgInvoke : forall r t f (Hbody : in_denotational_sem_goal (proj1_sig (MiniKanrenSyntax.P r) t) f),
+| dsgInvoke : forall r t f (DSG : in_denotational_sem_goal (proj1_sig (MiniKanrenSyntax.P r) t) f),
                            in_denotational_sem_goal (Invoke r t) f.
 
 Hint Constructors in_denotational_sem_goal.
 
 Inductive in_denotational_sem_lev_goal : nat -> goal -> gt_fun -> Prop :=
-| dslgUnify  : forall l f t1 t2 (UnH : gt_eq (apply_gt_fun f t1) (apply_gt_fun f t2)),
+| dslgCut    : forall l f, in_denotational_sem_lev_goal (S l) Cut f
+| dslgUnify  : forall l f t1 t2 (UNI : gt_eq (apply_gt_fun f t1) (apply_gt_fun f t2)),
                                 in_denotational_sem_lev_goal (S l) (Unify t1 t2) f
-| dslgDisjL  : forall l f g1 g2 (Hg :in_denotational_sem_lev_goal l g1 f),
+| dslgDisjL  : forall l f g1 g2 (DSG : in_denotational_sem_lev_goal l g1 f),
                                 in_denotational_sem_lev_goal l (Disj g1 g2) f
-| dslgDisjR  : forall l f g1 g2 (Hg :in_denotational_sem_lev_goal l g2 f),
+| dslgDisjR  : forall l f g1 g2 (DSG : in_denotational_sem_lev_goal l g2 f),
                                 in_denotational_sem_lev_goal l (Disj g1 g2) f
-| dslgConj   : forall l f g1 g2 (Hg1 :in_denotational_sem_lev_goal l g1 f)
-                                (Hg2 :in_denotational_sem_lev_goal l g2 f),
+| dslgConj   : forall l f g1 g2 (DSG_L : in_denotational_sem_lev_goal l g1 f)
+                                (DSG_R : in_denotational_sem_lev_goal l g2 f),
                                 in_denotational_sem_lev_goal l (Conj g1 g2) f
-| dslgFresh  : forall l f fn a fg (fvH : ~ is_fv_of_goal a (Fresh fg))
-                                  (Hg :in_denotational_sem_lev_goal l (fg a) fn)
-                                  (Hease : forall (x : name) (neq : x <> a), gt_eq (fn x) (f x)),
+| dslgFresh  : forall l f fn a fg (A_NOT_FV : ~ is_fv_of_goal a (Fresh fg))
+                                  (DSG : in_denotational_sem_lev_goal l (fg a) fn)
+                                  (EASE : forall (x : name) (neq : x <> a), gt_eq (fn x) (f x)),
                                   in_denotational_sem_lev_goal l (Fresh fg) f
-| dslgInvoke : forall l r t f (Hbody :in_denotational_sem_lev_goal l (proj1_sig (MiniKanrenSyntax.P r) t) f),
+| dslgInvoke : forall l r t f (DSG : in_denotational_sem_lev_goal l (proj1_sig (MiniKanrenSyntax.P r) t) f),
                               in_denotational_sem_lev_goal (S l) (Invoke r t) f.
 
 Hint Constructors in_denotational_sem_lev_goal.
 
-Lemma in_denotational_sem_zero_lev (g : goal)
-                                   (f : gt_fun) :
-                                   ~ in_denotational_sem_lev_goal 0 g f.
+Lemma in_denotational_sem_zero_lev
+      (g : goal)
+      (f : gt_fun) :
+      ~ in_denotational_sem_lev_goal 0 g f.
 Proof.
   intro. remember 0 as l. induction H; inversion Heql; auto.
 Qed.
 
-Lemma in_denotational_sem_lev_monotone (l : nat)
-                                       (g : goal)
-                                       (f : gt_fun)
-                                       (Hdsg : in_denotational_sem_lev_goal l g f)
-                                       (l' : nat)
-                                       (Hle: l <= l')
-                                       : in_denotational_sem_lev_goal l' g f.
+Lemma in_denotational_sem_lev_monotone
+      (l : nat)
+      (g : goal)
+      (f : gt_fun)
+      (DSG : in_denotational_sem_lev_goal l g f)
+      (l' : nat)
+      (LE: l <= l')
+      : in_denotational_sem_lev_goal l' g f.
 Proof.
-  revert Hle. revert l'. induction Hdsg; eauto.
-  { intros. destruct l'; auto. inversion Hle. }
+  revert LE. revert l'. induction DSG; eauto.
+  1-2: intros; destruct l'; auto; inversion LE.
   { intros. destruct l'.
-    { inversion Hle. }
-    { apply le_S_n in Hle. auto. } }
+    { inversion LE. }
+    { apply le_S_n in LE. auto. } }
 Qed.
 
-Lemma in_denotational_sem_some_lev (g : goal)
-                                   (f : gt_fun)
-                                   (Hdsg : in_denotational_sem_goal g f) :
-                                   exists l, in_denotational_sem_lev_goal l g f.
+Lemma in_denotational_sem_some_lev
+      (g : goal)
+      (f : gt_fun)
+      (DSG : in_denotational_sem_goal g f) :
+      exists l, in_denotational_sem_lev_goal l g f.
 Proof.
-  induction Hdsg.
-  { exists 1. auto. }
-  { destruct IHHdsg. eauto. }
-  { destruct IHHdsg. eauto. }
-  { destruct IHHdsg1. destruct IHHdsg2.
+  induction DSG.
+  1-2: exists 1; auto.
+  1-2, 4-5: destruct IHDSG; eauto.
+  { destruct IHDSG1. destruct IHDSG2.
     exists (max x x0). constructor.
     { eapply in_denotational_sem_lev_monotone; eauto. apply PeanoNat.Nat.le_max_l. }
     { eapply in_denotational_sem_lev_monotone; eauto. apply PeanoNat.Nat.le_max_r. } }
-  { destruct IHHdsg. eauto. }
-  { destruct IHHdsg. eauto. }
 Qed.
 
 Lemma den_sem_fv_only
       (f f' : gt_fun)
       (g : goal)
       (l : nat)
-      (ff'_eq : forall x, is_fv_of_goal x g -> gt_eq (f x) (f' x))
-      (Hgoal : in_denotational_sem_lev_goal l g f) :
+      (FF'_EQ : forall x, is_fv_of_goal x g -> gt_eq (f x) (f' x))
+      (DSG : in_denotational_sem_lev_goal l g f) :
       in_denotational_sem_lev_goal l g f'.
 Proof.
-  revert ff'_eq. revert f'. induction Hgoal; intros.
+  revert FF'_EQ. revert f'. induction DSG; intros.
+  { constructor. }
   { constructor. assert (gt_eq (apply_gt_fun f t1) (apply_gt_fun f' t1)).
     { apply apply_gt_fun_fv. auto. }
     assert (gt_eq (apply_gt_fun f t2) (apply_gt_fun f' t2)).
     { apply apply_gt_fun_fv. auto. }
-    revert UnH H H0. unfold gt_eq. intros. congruence. }
-  { constructor. apply IHHgoal. intros.
-    apply ff'_eq. auto. }
-  { apply dslgDisjR. apply IHHgoal. intros.
-    apply ff'_eq. auto. }
+    revert UNI H H0. unfold gt_eq. intros. congruence. }
+  { constructor. apply IHDSG. intros.
+    apply FF'_EQ. auto. }
+  { apply dslgDisjR. apply IHDSG. intros.
+    apply FF'_EQ. auto. }
   { constructor.
-    { apply IHHgoal1; intros; apply ff'_eq; auto. }
-    { apply IHHgoal2; intros; apply ff'_eq; auto. } }
+    { apply IHDSG1; intros; apply FF'_EQ; auto. }
+    { apply IHDSG2; intros; apply FF'_EQ; auto. } }
   { remember (fun x => if name_eq_dec x a
                          then fn a
                          else f' x) as fn'.
     apply dslgFresh with fn' a; auto.
-    { apply IHHgoal. intros. rewrite Heqfn'.
+    { apply IHDSG. intros. rewrite Heqfn'.
       destruct (name_eq_dec x a).
       { unfold gt_eq. subst. auto. }
-      { specialize (Hease _ n). red. rewrite Hease.
-        apply ff'_eq. eauto. } }
+      { specialize (EASE _ n). red. rewrite EASE.
+        apply FF'_EQ. eauto. } }
     { rewrite Heqfn'. intros.
       destruct (name_eq_dec x a); try contradiction.
       reflexivity. } }
-  { constructor. apply IHHgoal. intros.
-    apply ff'_eq. constructor.
+  { constructor. apply IHDSG. intros.
+    apply FF'_EQ. constructor.
     remember (MiniKanrenSyntax.P r). destruct d as [rel [Hcl Hco]].
     simpl in H. red in Hcl. red in Hcl. auto. }
 Qed.
 
-
 Lemma den_sem_rename_var
       (g1 g2 : goal)
-      (cg_g : consistent_goal g1)
+      (CG : consistent_goal g1)
       (n : nat)
-      (g1Bound : forall x : name, is_fv_of_goal x g1 -> x < n)
-      (g2Bound : forall x : name, is_fv_of_goal x g2 -> x < n)
+      (G1_BOUND : forall x : name, is_fv_of_goal x g1 -> x < n)
+      (G2_BOUND : forall x : name, is_fv_of_goal x g2 -> x < n)
       (a1 a2 : name)
-      (a12_neq : a1 <> a2)
-      (a2_fresh : ~ is_fv_of_goal a2 g1)
-      (sar : semiadequate_renaming a1 a2 g1 g2)
+      (A12_NEQ : a1 <> a2)
+      (A2_FRESH : ~ is_fv_of_goal a2 g1)
+      (REN : renaming a1 a2 g1 g2)
       (fa1 fa2 : gt_fun)
       (l : nat)
-      (Hgoal_f1 : in_denotational_sem_lev_goal l g1 fa1)
-      (f_switch : gt_eq (fa1 a1) (fa2 a2))
-      (f12_eq : forall x, x <> a1 -> x <> a2 -> gt_eq (fa1 x) (fa2 x)) :
+      (DSG1 : in_denotational_sem_lev_goal l g1 fa1)
+      (F_SWITCH : gt_eq (fa1 a1) (fa2 a2))
+      (F12_EQ : forall x, x <> a1 -> x <> a2 -> gt_eq (fa1 x) (fa2 x)) :
       in_denotational_sem_lev_goal l g2 fa2.
 Proof.
-  revert cg_g g1Bound g2Bound a12_neq a2_fresh sar Hgoal_f1 f_switch f12_eq.
+  revert CG G1_BOUND G2_BOUND A12_NEQ A2_FRESH REN DSG1 F_SWITCH F12_EQ.
   revert g1 g2 n a1 a2 fa1 fa2.
   induction l.
-  { intros. apply in_denotational_sem_zero_lev in Hgoal_f1. contradiction. }
-  { induction g1; intros; good_inversion Hgoal_f1; good_inversion sar; good_inversion cg_g.
+  { intros. apply in_denotational_sem_zero_lev in DSG1. contradiction. }
+  { induction g1; intros; good_inversion DSG1; good_inversion REN; good_inversion CG.
+    { constructor. }
     { constructor.
       etransitivity.
       2: etransitivity.
-      2: apply UnH.
+      2: apply UNI.
       1-2: etransitivity.
       1, 3: symmetry.
       1, 4: apply gt_fun_apply_compose.
       all: apply apply_gt_fun_fv; intros; unfold subst_gt_fun_compose;
         simpl; destruct (Nat.eq_dec a1 x); subst; symmetry; auto;
-        apply f12_eq; auto; intro; subst; auto. }
+        apply F12_EQ; auto; intro; subst; auto. }
     { apply dslgDisjL; eauto. eapply IHg1_1; eauto. }
     { apply dslgDisjR; eauto. eapply IHg1_2; eauto. }
     { constructor; eauto.
       { eapply IHg1_1; eauto. }
       { eapply IHg1_2; eauto. } }
     { apply den_sem_fv_only with fa1.
-      { intros; apply f12_eq; intro; subst; auto. }
+      { intros; apply F12_EQ; intro; subst; auto. }
       { econstructor.
         2: eauto.
         all: eauto. } }
-    { rename g into fg. rename fn into fn1. rename a into a0. red in HBinding.
+    { rename g into fg. rename fn into fn1. rename a into a0. red in CB_FG.
       assert (very_fresh_var : exists y, a0 <> y /\ a2 <> y /\
                                          (~ is_fv_of_goal y (Fresh fg)) /\
                                          (~ is_fv_of_goal y (Fresh rfg))).
@@ -336,7 +347,7 @@ Proof.
         1, 3, 9: exists (S n).
         4, 5: exists (S (S n)).
         all: repeat split; try omega.
-        all: intro CH; try apply g1Bound in CH; try apply g2Bound in CH; omega. }
+        all: intro CH; try apply G1_BOUND in CH; try apply G2_BOUND in CH; omega. }
       destruct very_fresh_var as [a3 [a03_neq [a23_neq [a3_fresh a3_rfresh]]]].
       assert (a13_neq : a1 <> a3).
       { intro; subst; auto. }
@@ -390,7 +401,7 @@ Proof.
         { destruct (name_eq_dec a1 a3); subst.
           { contradiction. }
           { etransitivity.
-            { apply Hease. auto. }
+            { apply EASE. auto. }
             { auto. } } } }
       { destruct (name_eq_dec x a1); subst.
         { reflexivity. }
@@ -399,8 +410,8 @@ Proof.
           { destruct (name_eq_dec x a0); subst.
             { reflexivity. }
             { etransitivity.
-              { apply Hease. auto. }
-              { apply f12_eq; auto. } } } } } }
+              { apply EASE. auto. }
+              { apply F12_EQ; auto. } } } } } }
     { rename n into r. rename n0 into n.
       remember (MiniKanrenSyntax.P r) as d. destruct d as [rel [Hcl Hco]].
       red in Hco. destruct (Hco t) as [Hcog Hcof].
@@ -414,23 +425,23 @@ Qed.
 
 Lemma den_sem_another_fresh_var
       (b : name -> goal)
-      (cg : consistent_goal (Fresh b))
+      (CG : consistent_goal (Fresh b))
       (n : nat)
-      (freshBound : forall x : name, is_fv_of_goal x (Fresh b) -> x < n)
+      (FRESH_BOUND : forall x : name, is_fv_of_goal x (Fresh b) -> x < n)
       (a1 a2 : name)
-      (a1_fresh : ~ is_fv_of_goal a1 (Fresh b))
-      (a2_fresh : ~ is_fv_of_goal a2 (Fresh b))
+      (A1_FRESH : ~ is_fv_of_goal a1 (Fresh b))
+      (A2_FRESH : ~ is_fv_of_goal a2 (Fresh b))
       (fa1 fa2 : gt_fun)
       (l : nat)
-      (Hgoal_f1 : in_denotational_sem_lev_goal l (b a1) fa1)
-      (f_switch : gt_eq (fa1 a1) (fa2 a2))
-      (f12_eq : forall x, x <> a1 -> x <> a2 -> gt_eq (fa1 x) (fa2 x)) :
+      (DSG1 : in_denotational_sem_lev_goal l (b a1) fa1)
+      (F_SWITCH : gt_eq (fa1 a1) (fa2 a2))
+      (F12_EQ : forall x, x <> a1 -> x <> a2 -> gt_eq (fa1 x) (fa2 x)) :
       in_denotational_sem_lev_goal l (b a2) fa2.
 Proof.
   destruct (name_eq_dec a1 a2); subst.
   { apply den_sem_fv_only with fa1; auto.
     intros. destruct (name_eq_dec x a2); subst; auto. }
-  { good_inversion cg. red in HBinding.
+  { good_inversion CG. red in CB_FG.
     eapply den_sem_rename_var with (g1 := (b a1)) (n := max n (max (S a1) (S a2))); eauto.
     { intros. destruct (name_eq_dec x a1); subst.
       { zify. omega. }
