src/MiniKanrenSyntax.v
@@ -1,50 +1,50 @@
+Add LoadPath "~/JB/minikanren-coq/src/".
+
 Require Import List.
 Import ListNotations.
 Require Import Coq.Lists.ListSet.
 Require Import Arith.
 Require Import Omega.
-Require Eqdep_dec Arith.
 Require Import Unify.
 
 Inductive goal : Set :=
-(* failure     *) | Fail   : goal
-(* unification *) | Unify  : term -> term -> goal
-(* disjunction *) | Disj   : goal -> goal -> goal
-(* conjunction *) | Conj   : goal -> goal -> goal
-(* fresh       *) | Fresh  : (name -> goal) -> goal
-(* invoke      *) | Invoke : name -> term -> goal.
+| Fail   : goal
+| Cut    : goal
+| Unify  : term -> term -> goal
+| Disj   : goal -> goal -> goal
+| Conj   : goal -> goal -> goal
+| Fresh  : (name -> goal) -> goal
+| Invoke : name -> term -> goal.
 
 (* rel is a body of a relational symbol *)
 Definition rel : Set := term -> goal.
 
 Inductive is_fv_of_goal (n : name) : goal -> Prop :=
-| fvUnifyL : forall t1 t2 (HInFv : In n (fv_term t1)),
+| fvUnifyL : forall t1 t2 (IN_FV : In n (fv_term t1)),
                           is_fv_of_goal n (Unify t1 t2)
-| fvUnifyR : forall t1 t2 (HInFv : In n (fv_term t2)),
+| fvUnifyR : forall t1 t2 (IN_FV : In n (fv_term t2)),
                           is_fv_of_goal n (Unify t1 t2)
-| fvDisjL  : forall g1 g2 (HisFV : is_fv_of_goal n g1),
+| fvDisjL  : forall g1 g2 (IS_FV : is_fv_of_goal n g1),
                           is_fv_of_goal n (Disj g1 g2)
-| fvDisjR  : forall g1 g2 (HisFV : is_fv_of_goal n g2),
+| fvDisjR  : forall g1 g2 (IS_FV : is_fv_of_goal n g2),
                           is_fv_of_goal n (Disj g1 g2)
-| fvConjL  : forall g1 g2 (HisFV : is_fv_of_goal n g1),
+| fvConjL  : forall g1 g2 (IS_FV : is_fv_of_goal n g1),
                           is_fv_of_goal n (Conj g1 g2)
-| fvConjR  : forall g1 g2 (HisFV : is_fv_of_goal n g2),
+| fvConjR  : forall g1 g2 (IS_FV : is_fv_of_goal n g2),
                           is_fv_of_goal n (Conj g1 g2)
-| fvFresh  : forall fg n' (neq : n' <> n)
-                          (HisFV : is_fv_of_goal n (fg n')),
+| fvFresh  : forall fg n' (NEQ : n' <> n)
+                          (IS_FV : is_fv_of_goal n (fg n')),
                           is_fv_of_goal n (Fresh fg)
-| fvInvoke : forall r arg (HInFv : In n (fv_term arg)),
+| fvInvoke : forall r arg (IN_FV : In n (fv_term arg)),
                           is_fv_of_goal n (Invoke r arg).
 
 Hint Constructors is_fv_of_goal.
 
-(* Closedness of goals *)
 Definition closed_goal_in_context (c : list name) (g : goal) : Prop :=
   forall n, is_fv_of_goal n g -> In n c.
 
 Definition closed_goal : goal -> Prop := closed_goal_in_context [].
 
-(* Closedness of a relational symbol *)
 Definition closed_rel (r : rel) : Prop :=
   forall (arg : term), closed_goal_in_context (fv_term arg) (r arg).
 
@@ -56,15 +56,15 @@ Module SmokeTest.
 
   Lemma g0_closed : closed_goal g0.
   Proof.
-    red. red. intros. inversion H. inversion HisFV.
-    { simpl in HInFv. destruct HInFv; contradiction. }
-    { inversion HInFv. }
+    red. red. intros. inversion H. inversion IS_FV.
+    { simpl in IN_FV. destruct IN_FV; contradiction. }
+    { inversion IN_FV. }
   Qed.
 
   Lemma g1_closed : closed_goal g1.
   Proof.
-    red. red. intros. inversion H. inversion HisFV.
-    inversion HisFV0; inversion HInFv; contradiction.
+    red. red. intros. inversion H. inversion IS_FV.
+    inversion IS_FV0; inversion IN_FV; contradiction.
   Qed.
 
   Definition r0 : rel := (fun t => Fresh (fun x => Fresh (fun y =>
@@ -73,16 +73,16 @@ Module SmokeTest.
 
   Lemma r0_closed : closed_rel r0.
   Proof.
-    red. red. intros. inversion H. inversion HisFV.
-    inversion HisFV0.
-    { inversion HisFV; auto. inversion HisFV2; inversion HisFV3.
+    red. red. intros. inversion H. inversion IS_FV.
+    inversion IS_FV0.
+    { inversion IS_FV; auto. inversion IS_FV2; inversion IS_FV3.
       { auto. }
-      { simpl in HInFv. destruct (name_eq_dec n'1 n').
-        { inversion HInFv; contradiction. }
-        { inversion HInFv; try contradiction. inversion H0; contradiction. } }
-      { inversion HInFv; contradiction. }
-      { inversion HInFv; contradiction. } }
-    { inversion HisFV1; inversion HInFv; contradiction. }
+      { simpl in IN_FV. destruct (name_eq_dec n'1 n').
+        { inversion IN_FV; contradiction. }
+        { inversion IN_FV; try contradiction. inversion H0; contradiction. } }
+      { inversion IN_FV; contradiction. }
+      { inversion IN_FV; contradiction. } }
+    { inversion IS_FV1; inversion IN_FV; contradiction. }
   Qed.
 
   Lemma r1_non_closed : ~ closed_rel r1.
@@ -96,56 +96,58 @@ Module SmokeTest.
 
 End SmokeTest.
 
-Inductive semiadequate_renaming (old_x : name) (new_x : name) : goal -> goal -> Prop :=
-| sarFail : semiadequate_renaming old_x new_x Fail Fail
-| sarUnify : forall t1 t2, semiadequate_renaming old_x new_x (Unify t1 t2)
-                                                 (Unify (apply_subst [(old_x, Var new_x)] t1)
-                                                        (apply_subst [(old_x, Var new_x)] t2))
-| sarDisj : forall g1 g2 rg1 rg2 (sar1 : semiadequate_renaming old_x new_x g1 rg1)
-                                 (sar2 : semiadequate_renaming old_x new_x g2 rg2),
-                                 semiadequate_renaming old_x new_x (Disj g1 g2) (Disj rg1 rg2)
-| sarConj : forall g1 g2 rg1 rg2 (sar1 : semiadequate_renaming old_x new_x g1 rg1)
-                                 (sar2 : semiadequate_renaming old_x new_x g2 rg2),
-                                 semiadequate_renaming old_x new_x (Conj g1 g2) (Conj rg1 rg2)
-| sarFreshNFV : forall fg (old_x_NFV : ~ is_fv_of_goal old_x (Fresh fg)),
-                          semiadequate_renaming old_x new_x (Fresh fg) (Fresh fg)
-| sarFreshFV : forall fg rfg (old_x_FV : is_fv_of_goal old_x (Fresh fg))
-                             (sar_fg : forall y (y_NFV : ~ is_fv_of_goal y (Fresh fg)), semiadequate_renaming old_x new_x (fg y) (rfg y)),
-                             semiadequate_renaming old_x new_x (Fresh fg) (Fresh rfg)
-| sarInvoke : forall r arg, semiadequate_renaming old_x new_x (Invoke r arg)
-                                                  (Invoke r (apply_subst [(old_x, Var new_x)] arg)).
+(* Weak version of a variable renaming *)
+Inductive renaming (old_x : name) (new_x : name) : goal -> goal -> Prop :=
+| rFail : renaming old_x new_x Fail Fail
+| rCut  : renaming old_x new_x Cut Cut
+| rUnify : forall t1 t2, renaming old_x new_x (Unify t1 t2)
+                                              (Unify (apply_subst [(old_x, Var new_x)] t1)
+                                                     (apply_subst [(old_x, Var new_x)] t2))
+| rDisj : forall g1 g2 rg1 rg2 (R_G1 : renaming old_x new_x g1 rg1)
+                               (R_G2 : renaming old_x new_x g2 rg2),
+                               renaming old_x new_x (Disj g1 g2) (Disj rg1 rg2)
+| rConj : forall g1 g2 rg1 rg2 (R_G1 : renaming old_x new_x g1 rg1)
+                               (R_G2 : renaming old_x new_x g2 rg2),
+                               renaming old_x new_x (Conj g1 g2) (Conj rg1 rg2)
+| rFreshNFV : forall fg (OLD_X_NOT_FV : ~ is_fv_of_goal old_x (Fresh fg)),
+                        renaming old_x new_x (Fresh fg) (Fresh fg)
+| rFreshFV : forall fg rfg (OLD_X_FV : is_fv_of_goal old_x (Fresh fg))
+                           (R_FG : forall y (Y_NOT_FV : ~ is_fv_of_goal y (Fresh fg)),
+                                            renaming old_x new_x (fg y) (rfg y)),
+                           renaming old_x new_x (Fresh fg) (Fresh rfg)
+| rInvoke : forall r arg, renaming old_x new_x (Invoke r arg)
+                                               (Invoke r (apply_subst [(old_x, Var new_x)] arg)).
 
-Hint Constructors semiadequate_renaming.
+Hint Constructors renaming.
 
 Definition consistent_binding (b : name -> goal) : Prop :=
-  forall x y, (~ is_fv_of_goal x (Fresh b)) -> semiadequate_renaming x y (b x) (b y).
+  forall x y, (~ is_fv_of_goal x (Fresh b)) -> renaming x y (b x) (b y).
 
 Inductive consistent_goal : goal -> Prop :=
 | cgFail   : consistent_goal Fail
+| cgCut    : consistent_goal Cut
 | cgUnify  : forall t1 t2, consistent_goal (Unify t1 t2)
-| cgDisj   : forall g1 g2 (Hcg1 : consistent_goal g1)
-                          (Hcg2 : consistent_goal g2),
+| cgDisj   : forall g1 g2 (CG_G1 : consistent_goal g1)
+                          (CG_G2 : consistent_goal g2),
                           consistent_goal (Disj g1 g2)
-| cgConj   : forall g1 g2 (Hcg1 : consistent_goal g1)
-                          (Hcg2 : consistent_goal g2),
+| cgConj   : forall g1 g2 (CG_G1 : consistent_goal g1)
+                          (CG_G2 : consistent_goal g2),
                           consistent_goal (Conj g1 g2)
-| cgFresh  : forall fg (HBinding : consistent_binding fg)
-                       (HcgInner : forall n, consistent_goal (fg n)),
+| cgFresh  : forall fg (CB_FG : consistent_binding fg)
+                       (CG_BODY : forall n, consistent_goal (fg n)),
                        consistent_goal (Fresh fg)
 | cgInvoke : forall r arg, consistent_goal (Invoke r arg).
 
 Hint Constructors consistent_goal.
 
 Definition consistent_function (f : term -> goal) : Prop :=
-  forall a1 a2 t, semiadequate_renaming a1 a2 (f t) (f (apply_subst [(a1, Var a2)] t)).
+  forall a1 a2 t, renaming a1 a2 (f t) (f (apply_subst [(a1, Var a2)] t)).
 
 Definition consistent_rel (r : rel) : Prop :=
   forall (arg : term), consistent_goal (r arg) /\ consistent_function r.
 
-(* def is a definition of a closed relational symbol *)
 Definition def : Set := {r : rel | closed_rel r /\ consistent_rel r}.
 
-(* spec is a list of definitions *)
 Definition spec : Set := name -> def.
 
 Variable P : spec.
