src/OperationalSem.v
@@ -1,9 +1,12 @@
+Add LoadPath "~/JB/minikanren-coq/src/".
+
 Require Import List.
 Require Import Coq.Lists.ListSet.
 Require Import Unify.
 Require Import MiniKanrenSyntax.
 Require Import Stream.
 Require Import Omega.
+Require Import Extraction.
 
 (* Partial state *) 
 Inductive state' : Set :=
@@ -17,46 +20,59 @@ Inductive state : Set :=
 (* a partial state   *) | State : state' -> state.
 
 Inductive is_fv_of_state' : name -> state' -> Prop :=
-| isfvst'Leaf  : forall x g s n     (isfvH : is_fv_of_goal x g),      is_fv_of_state' x (Leaf g s n)
-| isfvst'SumL  : forall x st'1 st'2 (isfvH : is_fv_of_state' x st'1), is_fv_of_state' x (Sum st'1 st'2)
-| isfvst'SumR  : forall x st'1 st'2 (isfvH : is_fv_of_state' x st'2), is_fv_of_state' x (Sum st'1 st'2)
-| isfvst'ProdL : forall x st' g     (isfvH : is_fv_of_state' x st'),  is_fv_of_state' x (Prod st' g)
-| isfvst'ProdR : forall x st' g     (isfvH : is_fv_of_goal x g),      is_fv_of_state' x (Prod st' g).
+| isfvst'Leaf  : forall x g s n     (X_FV_G : is_fv_of_goal x g),
+                                    is_fv_of_state' x (Leaf g s n)
+| isfvst'SumL  : forall x st'1 st'2 (X_FV : is_fv_of_state' x st'1),
+                                    is_fv_of_state' x (Sum st'1 st'2)
+| isfvst'SumR  : forall x st'1 st'2 (X_FV : is_fv_of_state' x st'2),
+                                    is_fv_of_state' x (Sum st'1 st'2)
+| isfvst'ProdL : forall x st' g     (X_FV : is_fv_of_state' x st'),
+                                    is_fv_of_state' x (Prod st' g)
+| isfvst'ProdR : forall x st' g     (X_FV : is_fv_of_goal x g),
+                                    is_fv_of_state' x (Prod st' g).
 
 Hint Constructors is_fv_of_state'.
 
 Inductive is_fv_of_state : name -> state -> Prop :=
-| isfvstC : forall x st' (isfv'H : is_fv_of_state' x st'), is_fv_of_state x (State st').
+| isfvstC : forall x st' (X_FV_ST' : is_fv_of_state' x st'),
+                         is_fv_of_state x (State st').
 
 Hint Constructors is_fv_of_state.
 
 Inductive is_counter_of_state' : nat -> state' -> Prop :=
-| iscst'Leaf  : forall g s n,                                            is_counter_of_state' n (Leaf g s n)
-| iscst'SumL  : forall n st'1 st'2 (iscH : is_counter_of_state' n st'1), is_counter_of_state' n (Sum st'1 st'2)
-| iscst'SumR  : forall n st'1 st'2 (iscH : is_counter_of_state' n st'2), is_counter_of_state' n (Sum st'1 st'2)
-| iscst'Prod  : forall n st' g     (iscH : is_counter_of_state' n st'),  is_counter_of_state' n (Prod st' g).
+| iscst'Leaf  : forall g s n,      is_counter_of_state' n (Leaf g s n)
+| iscst'SumL  : forall n st'1 st'2 (ISC : is_counter_of_state' n st'1),
+                                   is_counter_of_state' n (Sum st'1 st'2)
+| iscst'SumR  : forall n st'1 st'2 (ISC : is_counter_of_state' n st'2),
+                                   is_counter_of_state' n (Sum st'1 st'2)
+| iscst'Prod  : forall n st' g     (ISC : is_counter_of_state' n st'),
+                                   is_counter_of_state' n (Prod st' g).
 
 Hint Constructors is_counter_of_state'.
 
 Inductive well_formed_state' : state' -> Set :=
-| wfLeaf : forall g s frn   (domLTCounter : forall x, in_subst_dom s x -> x < frn)
-                            (vranLTCounter : forall x, in_subst_vran s x -> x < frn)
-                            (FVLTCounter : forall x, is_fv_of_goal x g -> x < frn),
+| wfLeaf : forall g s frn   (DOM_LT_COUNTER :  forall x (X_IN_DOM : in_subst_dom s x),
+                                                        x < frn)
+                            (VRAN_LT_COUNTER : forall x (X_IN_VRAN : in_subst_vran s x),
+                                                        x < frn)
+                            (FV_LT_COUNTER :   forall x (X_FV : is_fv_of_goal x g),
+                                                        x < frn),
                             well_formed_state' (Leaf g s frn)
-| wfSum  : forall st'1 st'2 (wfst'1 : well_formed_state' st'1)
-                            (wfst'2 : well_formed_state' st'2),
+| wfSum  : forall st'1 st'2 (WF_L : well_formed_state' st'1)
+                            (WF_R : well_formed_state' st'2),
                             well_formed_state' (Sum st'1 st'2)
-| wfProd : forall st' g     (wfst': well_formed_state' st')
-                            (FVLTCounter : forall x frn, is_counter_of_state' frn st' ->
-                                                         is_fv_of_goal x g ->
-                                                         x < frn),
+| wfProd : forall st' g     (WF_L : well_formed_state' st')
+                            (FV_LT_COUNTER : forall x frn (FRN_COUNTER : is_counter_of_state' frn st')
+                                                          (X_FV : is_fv_of_goal x g),
+                                                          x < frn),
                             well_formed_state' (Prod st' g).
 
 Hint Constructors well_formed_state'.
 
 Inductive well_formed_state : state -> Set :=
 | wfEmpty    : well_formed_state Stop
-| wfNonEmpty : forall st' (wfState : well_formed_state' st'), well_formed_state (State st').
+| wfNonEmpty : forall st' (wfState : well_formed_state' st'),
+                          well_formed_state (State st').
 
 Hint Constructors well_formed_state.
 
@@ -67,19 +83,28 @@ Inductive label : Set :=
 
 (* Transitions *)
 Inductive eval_step : state' -> label -> state -> Set :=
-| FailS        : forall           s    n, eval_step (Leaf Fail s n) Step Stop
-| UnifyFail    : forall t1 t2     s    n, unify (apply_subst s t1) (apply_subst s t2) None      -> eval_step (Leaf (Unify t1 t2) s n) Step Stop
-| UnifySuccess : forall t1 t2     s s' n, unify (apply_subst s t1) (apply_subst s t2) (Some s') -> eval_step (Leaf (Unify t1 t2) s n) (Answer (compose s s') n) Stop
-| DisjS        : forall g1 g2     s    n, eval_step (Leaf (Disj g1 g2) s n) Step (State (Sum (Leaf g1 s n) (Leaf g2 s n)))
-| ConjS        : forall g1 g2     s    n, eval_step (Leaf (Conj g1 g2) s n) Step (State (Prod (Leaf g1 s n) g2))
-| FreshS       : forall fg        s    n, eval_step (Leaf (Fresh fg) s n)   Step (State (Leaf (fg n) s (S n)))
-| InvokeS      : forall r arg     s    n, eval_step (Leaf (Invoke r arg) s n) Step (State (Leaf (proj1_sig (MiniKanrenSyntax.P r) arg) s n))
-| SumE         : forall st1 st2        l (H: eval_step st1 l  Stop), eval_step (Sum st1 st2) l (State st2)
-| SumNE        : forall st1 st1' st2   l, eval_step st1 l (State st1')             -> eval_step (Sum st1 st2) l (State (Sum st2 st1'))
-| ProdSE       : forall st g            , eval_step st     Step         Stop       -> eval_step (Prod st g) Step Stop
-| ProdAE       : forall st g s n        , eval_step st    (Answer s n)  Stop       -> eval_step (Prod st g) Step (State (Leaf g s n))
-| ProdSNE      : forall st g     st'    , eval_step st     Step        (State st') -> eval_step (Prod st g) Step (State (Prod st' g))
-| ProdANE      : forall st g s n st'    , eval_step st    (Answer s n) (State st') -> eval_step (Prod st g) Step (State (Sum (Leaf g s n) (Prod st' g))).
+| esFail         : forall           s    n, eval_step (Leaf Fail s n) Step Stop
+| esCut          : forall           s    n, eval_step (Leaf Cut s n)  (Answer s n) Stop
+| esUnifyFail    : forall t1 t2     s    n  (MGU : mgu (apply_subst s t1) (apply_subst s t2) None),
+                                            eval_step (Leaf (Unify t1 t2) s n) Step Stop
+| esUnifySuccess : forall t1 t2     s s' n  (MGU : mgu (apply_subst s t1) (apply_subst s t2) (Some s')),
+                                            eval_step (Leaf (Unify t1 t2) s n) (Answer (compose s s') n) Stop
+| esDisj         : forall g1 g2     s    n, eval_step (Leaf (Disj g1 g2) s n) Step (State (Sum (Leaf g1 s n) (Leaf g2 s n)))
+| esConj         : forall g1 g2     s    n, eval_step (Leaf (Conj g1 g2) s n) Step (State (Prod (Leaf g1 s n) g2))
+| esFresh        : forall fg        s    n, eval_step (Leaf (Fresh fg) s n)   Step (State (Leaf (fg n) s (S n)))
+| esInvoke       : forall r arg     s    n, eval_step (Leaf (Invoke r arg) s n) Step (State (Leaf (proj1_sig (MiniKanrenSyntax.P r) arg) s n))
+| esSumE         : forall st1 st2        l  (STEP_L : eval_step st1 l  Stop),
+                                            eval_step (Sum st1 st2) l (State st2)
+| esSumNE        : forall st1 st1' st2   l  (STEP_L : eval_step st1 l (State st1')),
+                                            eval_step (Sum st1 st2) l (State (Sum st2 st1'))
+| esProdSE       : forall st g              (STEP_L : eval_step st Step Stop),
+                                            eval_step (Prod st g) Step Stop
+| esProdAE       : forall st g s n          (STEP_L : eval_step st (Answer s n) Stop),
+                                            eval_step (Prod st g) Step (State (Leaf g s n))
+| esProdSNE      : forall st g     st'      (STEP_L : eval_step st Step (State st')),
+                                            eval_step (Prod st g) Step (State (Prod st' g))
+| esProdANE      : forall st g s n st'      (STEP_L : eval_step st (Answer s n) (State st')),
+                                            eval_step (Prod st g) Step (State (Sum (Leaf g s n) (Prod st' g))).
 
 Hint Constructors eval_step.
 
@@ -99,43 +124,43 @@ Lemma counter_in_next_state
       (st' st'_next : state')
       (l : label)
       (EV : eval_step st' l (State st'_next))
-      (Hisc_st' :  is_counter_of_state' n st'_next) :
+      (ISC_NEXT :  is_counter_of_state' n st'_next) :
       exists n', n' <= n /\ is_counter_of_state' n' st'.
 Proof.
   remember (State st'_next) as st.
-  revert Heqst Hisc_st'. revert st'_next.
+  revert Heqst ISC_NEXT. revert st'_next.
   induction EV; intros; good_inversion Heqst.
   { exists n. split.
     { constructor. }
-    { good_inversion Hisc_st'; good_inversion iscH; auto. } }
+    { good_inversion ISC_NEXT; good_inversion ISC; auto. } }
   { exists n. split.
     { constructor. }
-    { good_inversion Hisc_st'; good_inversion iscH; auto. } }
-  { good_inversion Hisc_st'. exists n0. split.
+    { good_inversion ISC_NEXT; good_inversion ISC; auto. } }
+  { good_inversion ISC_NEXT. exists n0. split.
     { repeat constructor. }
     { auto. } }
   { exists n. split.
     { constructor. }
-    { good_inversion Hisc_st'; auto. } }
+    { good_inversion ISC_NEXT; auto. } }
   { exists n. split.
     { constructor. }
     { auto. } }
-  { specialize (IHEV st1' eq_refl). good_inversion Hisc_st'.
+  { specialize (IHEV st1' eq_refl). good_inversion ISC_NEXT.
     { exists n. split.
       { constructor. }
       { auto. } }
-    { apply IHEV in iscH. destruct iscH as [n' [Hle iscH]].
+    { apply IHEV in ISC. destruct ISC as [n' [LE ISC]].
       exists n'; auto. } }
-  { good_inversion Hisc_st'. exists n0.
+  { good_inversion ISC_NEXT. exists n0.
     eapply counter_in_answer in EV. split; auto. }
-  { specialize (IHEV st' eq_refl). good_inversion Hisc_st'.
-    apply IHEV in iscH. destruct iscH as [n' [Hle iscH]].
-    exists n'; auto.  }
-  { specialize (IHEV st' eq_refl). good_inversion Hisc_st'.
-    { good_inversion iscH. exists n0.
+  { specialize (IHEV st' eq_refl). good_inversion ISC_NEXT.
+    apply IHEV in ISC. destruct ISC as [n' [LE ISC]].
+    exists n'; auto. }
+  { specialize (IHEV st' eq_refl). good_inversion ISC_NEXT.
+    { good_inversion ISC. exists n0.
       eapply counter_in_answer in EV. split; auto. }
-    { good_inversion iscH. apply IHEV in iscH0.
-      destruct iscH0 as [n' [Hle iscH]]. exists n'; auto. } }
+    { good_inversion ISC. apply IHEV in ISC0.
+      destruct ISC0 as [n' [LE ISC]]. exists n'; auto. } }
 Qed.
 
 Lemma well_formed_subst_in_answer
@@ -144,41 +169,41 @@ Lemma well_formed_subst_in_answer
       (n : nat)
       (st : state)
       (EV : eval_step st' (Answer s n) st)
-      (wf_st' : well_formed_state' st') :
+      (WF : well_formed_state' st') :
       (forall x, in_subst_dom s x -> x < n) /\ (forall x, in_subst_vran s x -> x < n).
 Proof.
-  remember (Answer s n). induction EV; good_inversion Heql; good_inversion wf_st'; auto.
-  assert (FVt1 : forall x, In x (fv_term (apply_subst s0 t1)) -> x < n).
-  { clear u s'. intros. induction t1.
+  remember (Answer s n). induction EV; good_inversion Heql; good_inversion WF; auto.
+  assert (FV_LT_N_1 : forall x, In x (fv_term (apply_subst s0 t1)) -> x < n).
+  { clear MGU s'. intros. induction t1.
     { simpl in H. destruct (image s0 n0) eqn:eq; auto.
-      apply vranLTCounter. red. eauto. }
+      apply VRAN_LT_COUNTER. red. eauto. }
     { good_inversion H. }
     { simpl in H. apply (set_union_elim name_eq_dec) in H. destruct H.
-      { apply IHt1_1; auto. intros. apply FVLTCounter.
-        good_inversion H0; auto. apply fvUnifyL. simpl.
+      { apply IHt1_1; auto. intros. apply FV_LT_COUNTER.
+        good_inversion X_FV; auto. apply fvUnifyL. simpl.
         apply set_union_intro. left. auto. }
-      { apply IHt1_2; auto. intros. apply FVLTCounter.
-        good_inversion H0; auto. apply fvUnifyL. simpl.
+      { apply IHt1_2; auto. intros. apply FV_LT_COUNTER.
+        good_inversion X_FV; auto. apply fvUnifyL. simpl.
         apply set_union_intro. right. auto. } } }
-  assert (FVt2 : forall x, In x (fv_term (apply_subst s0 t2)) -> x < n).
-  { clear u s'. intros. induction t2.
+  assert (FV_LT_N_2 : forall x, In x (fv_term (apply_subst s0 t2)) -> x < n).
+  { clear MGU s'. intros. induction t2.
     { simpl in H. destruct (image s0 n0) eqn:eq; auto.
-      apply vranLTCounter. red. eauto. }
+      apply VRAN_LT_COUNTER. red. eauto. }
     { good_inversion H. }
     { simpl in H. apply (set_union_elim name_eq_dec) in H. destruct H.
-      { apply IHt2_1; auto. intros. apply FVLTCounter.
-        good_inversion H0; auto. apply fvUnifyR. simpl.
+      { apply IHt2_1; auto. intros. apply FV_LT_COUNTER.
+        good_inversion X_FV; auto. apply fvUnifyR. simpl.
         apply set_union_intro. left. auto. }
-      { apply IHt2_2; auto. intros. apply FVLTCounter.
-        good_inversion H0; auto. apply fvUnifyR. simpl.
+      { apply IHt2_2; auto. intros. apply FV_LT_COUNTER.
+        good_inversion X_FV; auto. apply fvUnifyR. simpl.
         apply set_union_intro. right. auto. } } }
-  specialize (MGU_dom _ _ _ u). intro s'Dom.
-  specialize (MGU_vran _ _ _ u). intro s'VRan.
+  specialize (mgu_dom _ _ _ MGU). intro S'_DOM.
+  specialize (mgu_vran _ _ _ MGU). intro S'_VRAN.
   split.
   { intros. apply compose_dom in H. destruct H; auto.
-    apply s'Dom in H. destruct H; auto. }
+    apply S'_DOM in H. destruct H; auto. }
   { intros. apply compose_vran in H. destruct H; auto.
-    apply s'VRan in H. destruct H; auto. }
+    apply S'_VRAN in H. destruct H; auto. }
 Qed.
 
 Lemma well_formedness_preservation
@@ -186,80 +211,87 @@ Lemma well_formedness_preservation
       (l : label)
       (st : state)
       (EV : eval_step st' l st)
-      (wf_st' : well_formed_state' st') :
+      (WF : well_formed_state' st') :
       well_formed_state st.
 Proof.
-  intros. induction EV; good_inversion wf_st'; auto.
+  intros. induction EV; good_inversion WF; auto.
   { constructor. auto. }
   { constructor. constructor; auto.
-    intros. good_inversion H. subst. auto. }
+    intros. good_inversion FRN_COUNTER. subst. auto. }
   { constructor. constructor.
     1-2: intros; eapply lt_trans; eauto.
     intros. destruct (eq_nat_dec n x).
     { omega. }
-    { apply Nat.lt_lt_succ_r. apply FVLTCounter. econstructor; eauto. } }
+    { apply Nat.lt_lt_succ_r. apply FV_LT_COUNTER. econstructor; eauto. } }
   { constructor. constructor; auto.
-    specialize (proj2_sig (MiniKanrenSyntax.P r)). intro Hcc.
-    simpl in Hcc. destruct Hcc as [Hcl _]. red in Hcl. red in Hcl. auto. }
-  { specialize (IHEV wfst'1).
+    specialize (proj2_sig (MiniKanrenSyntax.P r)). intro CC.
+    simpl in CC. destruct CC as [CL _]. red in CL. red in CL. auto. }
+  { specialize (IHEV WF_L).
     good_inversion IHEV. auto. }
   { constructor. constructor.
     1-2: apply well_formed_subst_in_answer in EV; destruct EV; auto.
-    intros. apply FVLTCounter; auto. eapply counter_in_answer; eauto. }
-  { specialize (IHEV wfst'). good_inversion IHEV.
+    intros. apply FV_LT_COUNTER; auto. eapply counter_in_answer; eauto. }
+  { specialize (IHEV WF_L). good_inversion IHEV.
     constructor. constructor; auto. intros.
     eapply counter_in_next_state in EV; eauto.
-    destruct EV as [frn' [Hle Hisc]]. eapply lt_le_trans.
+    destruct EV as [frn' [LE ISC]]. eapply lt_le_trans.
     2: eauto.
     auto. }
-  { specialize (IHEV wfst'). good_inversion IHEV.
+  { specialize (IHEV WF_L). good_inversion IHEV.
     constructor. constructor.
     { constructor.
       1-2: apply well_formed_subst_in_answer in EV; destruct EV; auto.
-      intros. apply FVLTCounter; auto.
+      intros. apply FV_LT_COUNTER; auto.
       eapply counter_in_answer; eauto. }
     { constructor; auto. intros.
       eapply counter_in_next_state in EV; eauto.
-      destruct EV as [frn' [Hle Hisc]]. eapply lt_le_trans.
+      destruct EV as [frn' [Le ISC]]. eapply lt_le_trans.
       2: eauto.
       auto. } }
 Qed.
 
-Lemma eval_step_exists : forall (st' : state'), {l : label & {st : state & eval_step st' l st}}.
+Lemma eval_step_exists
+      (st' : state') :
+      {l : label & {st : state & eval_step st' l st}}.
 Proof.
   induction st'.
-  * destruct g.
-    1,3-6: repeat eexists; econstructor.
-    + assert ({r & unify (apply_subst s t) (apply_subst s t0) r}). { apply unify_exists. }
+  { destruct g.
+    1-2,4-7: repeat eexists; econstructor.
+    { assert ({r & mgu (apply_subst s t) (apply_subst s t0) r}).
+      { apply mgu_exists. }
       destruct H. destruct x.
-      all: repeat eexists; eauto.
-  * destruct IHst'1 as [l1 [st1 IH1]]. destruct st1.
-    all: repeat eexists; eauto.
-  * destruct IHst' as [l [st IH]]. destruct st; destruct l.
-    all: repeat eexists; eauto.
+      all: repeat eexists; eauto. } }
+  { destruct IHst'1 as [l1 [st1 IH1]]. destruct st1.
+    all: repeat eexists; eauto. }
+  { destruct IHst' as [l [st IH]]. destruct st; destruct l.
+    all: repeat eexists; eauto. }
 Qed.
 
-Lemma eval_step_unique :
-  forall (st' : state') (l1 l2 : label) (st1 st2 : state),
-    eval_step st' l1 st1 -> eval_step st' l2 st2 -> l1 = l2 /\ st1 = st2.
+Lemma eval_step_unique
+      (st' : state')
+      (l1 l2 : label)
+      (st1 st2 : state)
+      (STEP_1 : eval_step st' l1 st1)
+      (STEP_2 : eval_step st' l2 st2) :
+      l1 = l2 /\ st1 = st2.
 Proof.
-  induction st'.
-  * intros. destruct g; inversion H; inversion H0; subst; auto.
-    + assert (C : None = Some s').
-      { eapply unify_unique; eassumption. }
-      inversion C.
-    + assert (C : None = Some s').
-      { eapply unify_unique; eassumption. }
-      inversion C.
-    + assert (C : Some s' = Some s'0).
-      { eapply unify_unique; eassumption. }
-      inversion C. auto.
-  * intros. inversion H; inversion H0; subst;
-    specialize (IHst'1 _ _ _ _ H5 H10); inversion IHst'1;
-    inversion H2; subst; auto.
-  * intros. inversion H; inversion H0; subst;
-    specialize (IHst' _ _ _ _ H5 H10); inversion IHst'; subst;
-    inversion H1; inversion H2; auto.
+  revert STEP_1 STEP_2. revert l1 l2 st1 st2. induction st'.
+  { intros. destruct g; good_inversion STEP_1; good_inversion STEP_2; auto.
+    { assert (C : None = Some s').
+      { eapply mgu_unique; eassumption. }
+      inversion C. }
+    { assert (C : None = Some s').
+      { eapply mgu_unique; eassumption. }
+      inversion C. }
+    { assert (C : Some s' = Some s'0).
+      { eapply mgu_unique; eassumption. }
+      inversion C. auto. } }
+  { intros. good_inversion STEP_1; good_inversion STEP_2;
+    specialize (IHst'1 _ _ _ _ STEP_L STEP_L0); inversion IHst'1;
+    inversion H0; subst; auto. }
+  { intros. good_inversion STEP_1; good_inversion STEP_2;
+    specialize (IHst' _ _ _ _ STEP_L STEP_L0); inversion IHst'; subst;
+    inversion H; inversion H0; auto. }
 Qed.
 
 (* Traces *)
@@ -283,30 +315,43 @@ CoFixpoint trace_from (st : state) : trace :=
     end
   end.
 
-Lemma trace_from_correct : forall st, op_sem st (trace_from st).
+Lemma trace_from_correct 
+      (st : state) :
+      op_sem st (trace_from st).
 Proof.
-  cofix CIH. destruct st.
+  revert st. cofix CIH. destruct st.
   { rewrite helper_eq. simpl. constructor. }
   { rewrite helper_eq. simpl. destruct (eval_step_exists s).
-    destruct s0. econstructor. eauto. eauto. }
+    destruct s0. econstructor; eauto. }
 Qed.
 
-Lemma op_sem_exists (st : state) : {t : trace & op_sem st t}.
+Lemma op_sem_exists
+      (st : state) :
+      {t : trace & op_sem st t}.
 Proof.
   eexists. eapply trace_from_correct.
 Qed.
 
-Lemma op_sem_unique :
-  forall st t1 t2, op_sem st t1 -> op_sem st t2 -> equal_streams t1 t2.
+Extraction Language Haskell.
+
+Extraction "Users/rozplokhas/JB/minikanren-coq/extracted/interpreter.hs" op_sem_exists.
+
+Lemma op_sem_unique
+      (st : state)
+      (t1 t2 : trace)
+      (OP_1 : op_sem st t1)
+      (OP_2 : op_sem st t2) :
+      equal_streams t1 t2.
 Proof.
-  cofix CIH. intros. inversion H; inversion H0;
-  rewrite <- H1 in H3; inversion H3.
-  * constructor.
-  * subst.
+  revert OP_1 OP_2. revert t1 t2 st.
+  cofix CIH. intros. inversion OP_1; inversion OP_2;
+  rewrite <- H1 in H; inversion H.
+  { constructor. }
+  { subst.
     specialize (eval_step_unique _ _ _ _ _ EV EV0).
-    intro. destruct H1. constructor.
-    + auto.
-    + subst. eapply CIH; eauto.
+    intros [EQL EQST]. constructor.
+    { auto. }
+    { subst. eapply CIH; eauto. } }
 Qed.
 
 Lemma counter_in_trace
@@ -319,64 +364,72 @@ Lemma counter_in_trace
       n <= nr.
 Proof.
   remember (Leaf g s n) as st'.
-  assert (forall n', is_counter_of_state' n' st' -> n <= n').
+  assert (CNT_GE : forall n', is_counter_of_state' n' st' -> n <= n').
   { intros. subst. good_inversion H. auto. }
-  clear Heqst'. revert H OP. revert n st'.
+  clear Heqst'. revert CNT_GE OP. revert n st'.
   remember (Answer sr nr). induction HIn; intros; subst.
   { good_inversion OP. apply counter_in_answer in EV. auto. }
   { good_inversion OP. destruct st.
     { good_inversion OP0. good_inversion HIn. }
     { apply IHHIn with s0; auto. intros.
-      specialize (counter_in_next_state _ _ _ _ EV H0). intros.
-      destruct H1. destruct H1. apply H in H2.
+      specialize (counter_in_next_state _ _ _ _ EV H). intros.
+      destruct H0. destruct H0. apply CNT_GE in H1.
       eapply le_trans; eauto. } }
 Qed.
 
 Lemma well_formed_subst_in_trace
       (st : state)
-      (wf_st' : well_formed_state st)
+      (WF : well_formed_state st)
       (t : trace)
       (OP : op_sem st t)
       (s : subst)
       (n : nat)
-      (isAns: in_stream (Answer s n) t) :
+      (IS_ANS: in_stream (Answer s n) t) :
       (forall x, in_subst_dom s x -> x < n) /\ (forall x, in_subst_vran s x -> x < n).
 Proof.
-  remember (Answer s n). revert wf_st' OP. revert st.
-  induction isAns; intros.
-  { good_inversion OP. good_inversion wf_st'.
+  remember (Answer s n). revert WF OP. revert st.
+  induction IS_ANS; intros.
+  { good_inversion OP. good_inversion WF.
     eapply well_formed_subst_in_answer; eauto. }
-  { good_inversion OP. good_inversion wf_st'.
-    apply IHisAns with st0; auto.
+  { good_inversion OP. good_inversion WF.
+    apply IHIS_ANS with st0; auto.
     eapply well_formedness_preservation; eauto. }
 Qed.
 
-Lemma sum_op_sem : forall st'1 st'2 t1 t2 t, op_sem (State st'1) t1 ->
-                                             op_sem (State st'2) t2 ->
-                                             op_sem (State (Sum st'1 st'2)) t ->
-                                             interleave t1 t2 t.
+Lemma sum_op_sem
+      (st'1 st'2 : state')
+      (t1 t2 t : trace)
+      (OP_1 : op_sem (State st'1) t1)
+      (OP_2 : op_sem (State st'2) t2)
+      (OP_12 : op_sem (State (Sum st'1 st'2)) t) :
+      interleave t1 t2 t.
 Proof.
-  cofix CIH. intros. inversion H. subst. inversion H1. subst.
-  inversion EV0; subst; specialize (eval_step_unique _ _ _ _ _ EV H6);
-  intro; destruct H2; subst; constructor.
-  * inversion OP. subst. specialize (op_sem_unique _ _ _ H0 OP0).
-    intro. inversion H2; subst.
-    + constructor. constructor.
-    + constructor. constructor. auto.
-  * eapply CIH; eassumption.
+  revert OP_1 OP_2 OP_12. revert t1 t2 t st'1 st'2.
+  cofix CIH. intros. inversion OP_1. subst. inversion OP_12. subst.
+  inversion EV0; subst; specialize (eval_step_unique _ _ _ _ _ EV STEP_L);
+  intros [EQL EQST]; subst; constructor.
+  { inversion OP. subst. specialize (op_sem_unique _ _ _ OP_2 OP0).
+    intro EQS. inversion EQS; subst.
+    { constructor. constructor. }
+    { constructor. constructor. auto. } }
+  { eapply CIH; eassumption. }
 Qed.
 
-Lemma disjunction_finite_commutativity :
-  forall g1 g2 s n t12 t21
-    (ops11 : op_sem (State (Leaf (Disj g1 g2) s n)) t12)
-    (ops21 : op_sem (State (Leaf (Disj g2 g1) s n)) t21)
-    (fin12 : finite t12), finite t21.
+Lemma disjunction_finite_commutativity
+      (g1 g2 : goal)
+      (s : subst)
+      (n : nat)
+      (t12 t21 : trace)
+      (OP_12 : op_sem (State (Leaf (Disj g1 g2) s n)) t12)
+      (OP_21 : op_sem (State (Leaf (Disj g2 g1) s n)) t21)
+      (FIN_12 : finite t12) :
+      finite t21.
 Proof.
   intros.
-  inversion ops11; subst.
+  inversion OP_12; subst.
   inversion EV; subst.
-  inversion fin12; subst.
-  inversion ops21; subst.
+  inversion FIN_12; subst.
+  inversion OP_21; subst.
   inversion EV0; subst.
   constructor.
   specialize (op_sem_exists (State (Leaf g1 s n))). intro. destruct H as [t1 OP1].
@@ -384,8 +437,8 @@ Proof.
   specialize (sum_op_sem _ _ _ _ _ OP1 OP2 OP). intro.
   specialize (sum_op_sem _ _ _ _ _ OP2 OP1 OP0). intro.
   specialize (interleave_finite _ _ _ H). intro.
-  specialize (interleave_finite _ _ _ H1). intro.
-  apply H3. apply and_comm. apply H2. auto.
+  specialize (interleave_finite _ _ _ H0). intro.
+  apply H2. apply and_comm. apply H1. auto.
 Qed.
 
 Lemma prod_op_sem_in
@@ -398,14 +451,14 @@ Lemma prod_op_sem_in
       (OP : op_sem (State (Prod st' g)) t)
       (OP1 : op_sem (State st') t1)
       (OP2 : op_sem (State (Leaf g s n)) t2)
-      (HIn1 : in_stream (Answer s n) t1)
-      (HIn2 : in_stream r t2) :
+      (IN_1 : in_stream (Answer s n) t1)
+      (IN_2 : in_stream r t2) :
       in_stream r t.
 Proof.
   revert OP OP1. revert t st'. remember (Answer s n) as r1.
-  induction HIn1; intros; subst.
+  induction IN_1; intros; subst.
   { good_inversion OP1. good_inversion OP.
-    good_inversion EV0; specialize (eval_step_unique _ _ _ _ _ EV H3);
+    good_inversion EV0; specialize (eval_step_unique _ _ _ _ _ EV STEP_L);
     intro eqs; destruct eqs; subst; good_inversion H.
     { constructor. specialize (op_sem_unique _ _ _ OP2 OP1).
       intros. eapply in_equal_streams; eauto. }
@@ -417,17 +470,17 @@ Proof.
       intro interH. eapply interleave_in in interH.
       eapply interH. left. specialize (op_sem_unique _ _ _ OP2 OP3).
       intros. eapply in_equal_streams; eauto. } }
-  { specialize (IHHIn1 eq_refl).
+  { specialize (IHIN_1 eq_refl).
     good_inversion OP1. good_inversion OP.
-    good_inversion EV0; specialize (eval_step_unique _ _ _ _ _ EV H3);
+    good_inversion EV0; specialize (eval_step_unique _ _ _ _ _ EV STEP_L);
     intro eqs; destruct eqs; subst.
-    1-2: good_inversion OP0; good_inversion HIn1.
-    { constructor. eapply IHHIn1; eauto. }
+    1-2: good_inversion OP0; good_inversion IN_1.
+    { constructor. eapply IHIN_1; eauto. }
     { constructor. specialize (op_sem_exists (State (Leaf g s0 n0))).
       intro H. destruct H as [t3 OP3].
       specialize (op_sem_exists (State (Prod st'0 g))).
       intro H. destruct H as [t4 OP4].
       specialize (sum_op_sem _ _ _ _ _ OP3 OP4 OP1).
       intro interH. eapply interleave_in in interH.
-      eapply interH. right. eapply IHHIn1; eauto. } }
+      eapply interH. right. eapply IHIN_1; eauto. } }
 Qed.
