src/Unify.v
@@ -4,8 +4,6 @@ Require Import Arith.
 Require Import Omega.
 Require Import Coq.Lists.ListSet.
 Require Export Coq.Structures.OrderedTypeEx.
-Require Import Eqdep.
-Require Import Program.
 
 Ltac good_inversion H := inversion H; clear H; subst.
 
@@ -21,7 +19,7 @@ Inductive term : Set :=
 (* a constant           *) | Cst : name -> term
 (* a binary constructor *) | Con : name -> term -> term -> term.
 
-Lemma term_eq_dec : (forall t1 t2 : term, {t1 = t2} + {t1 <> t2}).
+Lemma term_eq_dec : forall t1 t2 : term, {t1 = t2} + {t1 <> t2}.
 Proof.
   induction t1; destruct t2.
   2, 3, 4, 6, 7, 8: right; intro H; inversion H.
@@ -52,36 +50,35 @@ Fixpoint fv_term (t : term) : var_set :=
 
 Definition ground_term : Set := {t : term | fv_term t = var_set_empty}.
 
-Lemma fv_term_nodup : forall t, NoDup (fv_term t).
+Lemma fv_term_nodup
+      (t : term) :
+      NoDup (fv_term t).
 Proof.
   induction t.
-  * apply set_add_nodup. constructor.
-  * constructor.
-  * apply set_union_nodup; assumption.
+  { apply set_add_nodup. constructor. }
+  { constructor. }
+  { apply set_union_nodup; assumption. }
 Qed.
 
-Definition fv_terms (ts : list term) : var_set :=
-  fold_left (fun acc t => var_set_union acc (fv_term t)) ts var_set_empty.
-
-Lemma free_var (t : term) : exists x, ~ In x (fv_term t).
+Lemma free_var
+      (t : term) :
+      exists x, ~ In x (fv_term t).
 Proof.
   assert (A : forall t, exists n, forall x, In x (fv_term t) -> S x <= n).
-  {
-    clear. induction t.
-    * exists (S n). intros. destruct H.
-      + omega.
-      + contradiction.
-    * exists 0. intros. contradiction.
-    * destruct IHt1 as [n1 IHt1]. destruct IHt2 as [n2 IHt2].
+  { clear. induction t.
+    { exists (S n). intros. destruct H.
+      { omega. }
+      { contradiction. } }
+    { exists 0. intros. contradiction. }
+    { destruct IHt1 as [n1 IHt1]. destruct IHt2 as [n2 IHt2].
       exists (max n1 n2). intros. apply (set_union_elim name_eq_dec) in H.
       destruct H.
-      + eapply le_trans.
-        - eapply IHt1. assumption.
-        - apply Nat.le_max_l.
-      + eapply le_trans.
-        - eapply IHt2. assumption.
-        - apply Nat.le_max_r.
-  }
+      { eapply le_trans.
+        { eapply IHt1. assumption. }
+        { apply Nat.le_max_l. } }
+      { eapply le_trans.
+        { eapply IHt2. assumption. }
+        { apply Nat.le_max_r. } } } }
   specialize (A t). destruct A. exists x. intro C.
   apply H in C. omega.
 Qed.
@@ -100,24 +97,27 @@ Fixpoint occurs (n : name) (t : term) : bool :=
   | Con _ l r => orb (occurs n l) (occurs n r)
   end.
 
-Lemma occurs_In: forall t n, occurs n t = true <-> In n (fv_term t).
+Lemma occurs_In
+      (t : term)
+      (n : name) :
+      occurs n t = true <-> In n (fv_term t).
 Proof.
-  intros. induction t.
-  * split; intro.
-    + left. symmetry. apply Nat.eqb_eq. assumption.
-    + destruct H.
-      - apply Nat.eqb_eq. symmetry. assumption.
-      - contradiction.
-  * split; intro C; inversion C.
-  * split; intro.
-    + apply (set_union_intro name_eq_dec).
+  induction t.
+  { split; intro.
+    { left. symmetry. apply Nat.eqb_eq. assumption. }
+    { destruct H.
+      { apply Nat.eqb_eq. symmetry. assumption. }
+      { contradiction. } } }
+  { split; intro C; inversion C. }
+  { split; intro.
+    { apply (set_union_intro name_eq_dec).
       apply Bool.orb_true_elim in H. destruct H.
-      - left. apply IHt1. assumption.
-      - right. apply IHt2. assumption.
-    + apply Bool.orb_true_intro.
+      { left. apply IHt1. assumption. }
+      { right. apply IHt2. assumption. } }
+    { apply Bool.orb_true_intro.
       apply (set_union_elim name_eq_dec) in H. destruct H.
-      - left. apply IHt1. assumption.
-      - right. apply IHt2. assumption.
+      { left. apply IHt1. assumption. }
+      { right. apply IHt2. assumption. } } }
 Qed.
 
 (******************** Substitutions **********************)
@@ -127,9 +127,6 @@ Definition subst : Set := list (name * term).
 Definition empty_subst : subst := [].
 
 Definition singleton_subst (n : name) (t : term) := [(n, t)].
-
-(* Substitution domain *)
-(* Definition domain (s : subst) : list name := nodup name_eq_dec (map (@fst name term) s). *)
 
 (* Substitution image *)
 Fixpoint image (s : subst) (n : name) : option term :=
@@ -142,14 +139,14 @@ Lemma map_image
       (f : name -> term)
       (v : var_set)
       (x : name)
-      (HIn : In x v) :
+      (X_IN : In x v) :
       image (map (fun x0 : name => (x0, f x0)) v) x = Some (f x).
 Proof.
   induction v.
   { contradiction. }
   { simpl. destruct (Nat.eq_dec a x).
     { subst. auto. }
-    { apply IHv. destruct HIn; auto. contradiction. } }
+    { apply IHv. destruct X_IN; auto. contradiction. } }
 Qed.
 
 Definition in_subst_dom (s : subst) (x : name) : Prop := exists t, image s x = Some t.
@@ -164,7 +161,9 @@ Fixpoint apply_subst (s : subst) (t : term) : term :=
   | Con n l r => Con n (apply_subst s l) (apply_subst s r)
   end.
 
-Lemma apply_empty: forall (t : term), apply_subst empty_subst t = t.
+Lemma apply_empty
+      (t : term) :
+      apply_subst empty_subst t = t.
 Proof.
   induction t; try (simpl; congruence); auto.
 Qed.
@@ -173,15 +172,15 @@ Lemma apply_subst_FV
       (x : name)
       (t : term)
       (s : subst)
-      (xFV : In x (fv_term (apply_subst s t))) :
+      (X_FV : In x (fv_term (apply_subst s t))) :
       In x (fv_term t) \/ in_subst_vran s x.
 Proof.
   induction t.
-  { simpl in xFV. destruct (image s n) eqn:eq.
+  { simpl in X_FV. destruct (image s n) eqn:eq.
     { right. red. eauto. }
     { left. auto. } }
-  { inversion xFV. }
-  { simpl in xFV. apply (set_union_elim name_eq_dec) in xFV. destruct xFV.
+  { inversion X_FV. }
+  { simpl in X_FV. apply (set_union_elim name_eq_dec) in X_FV. destruct X_FV.
     { apply IHt1 in H. destruct H.
       { left. apply (set_union_intro name_eq_dec). left. auto. }
       { right. auto. } }
@@ -190,38 +189,40 @@ Proof.
       { right. auto. } } }
 Qed.
 
-(* Composition *)
+(* Substitution composition *)
 Definition compose (s1 s2 : subst) : subst :=
   List.map (fun p => (fst p, apply_subst s2 (snd p))) s1 ++ s2.
 
-Lemma compose_correctness: forall (s1 s2 : subst) (t : term),
-  apply_subst (compose s1 s2) t = apply_subst s2 (apply_subst s1 t).
+Lemma compose_correctness
+      (s1 s2 : subst)
+      (t : term) :
+      apply_subst (compose s1 s2) t = apply_subst s2 (apply_subst s1 t).
 Proof.
-  intros. induction t.
-  * simpl. destruct (image s1 n) eqn:eq.
-    + induction s1.
-      - inversion eq.
-      - destruct a. simpl in eq. simpl. destruct (Nat.eq_dec n0 n).
+  induction t.
+  { simpl. destruct (image s1 n) eqn:eq.
+    { induction s1.
+      { inversion eq. }
+      { destruct a. simpl in eq. simpl. destruct (Nat.eq_dec n0 n).
         { congruence. }
-        { auto. }
-    + induction s1.
-      - reflexivity.
-      - destruct a. simpl in eq. simpl. destruct (Nat.eq_dec n0 n).
+        { auto. } } }
+    { induction s1.
+      { reflexivity. }
+      { destruct a. simpl in eq. simpl. destruct (Nat.eq_dec n0 n).
         { inversion eq. }
-        { auto. }
-  * reflexivity.
-  * simpl. congruence.
+        { auto. } } } }
+  { reflexivity. }
+  { simpl. congruence. }
 Qed.
 
 Lemma compose_dom
       (x : name)
       (s s' : subst)
-      (inDom : in_subst_dom (compose s s') x) :
+      (IN_DOM : in_subst_dom (compose s s') x) :
       in_subst_dom s x \/ in_subst_dom s' x.
 Proof.
   induction s.
   { right. auto. }
-  { red in inDom. destruct inDom. unfold in_subst_dom.
+  { red in IN_DOM. destruct IN_DOM. unfold in_subst_dom.
     simpl. destruct a. simpl in H.
     destruct (Nat.eq_dec n x).
     { left. eauto. }
@@ -231,18 +232,18 @@ Qed.
 Lemma compose_vran
       (y : name)
       (s s' : subst)
-      (inVRan : in_subst_vran (compose s s') y) :
+      (IN_VRAN : in_subst_vran (compose s s') y) :
       in_subst_vran s y \/ in_subst_vran s' y.
 Proof.
-  destruct inVRan as [x [t [inImage inFV]]].
-  assert (GenLemma : (exists t0, image s x = Some t0 /\ In y (fv_term t0)) \/ in_subst_vran s' y).
+  destruct IN_VRAN as [x [t [IN_IMAGE IN_FV]]].
+  assert (GEN : (exists t0, image s x = Some t0 /\ In y (fv_term t0)) \/ in_subst_vran s' y).
   { induction s.
     { right. red. eauto. }
-    { destruct a. simpl in inImage. simpl. destruct (Nat.eq_dec n x).
-      { inversion inImage. subst. apply apply_subst_FV in inFV.
-        destruct inFV; auto. left. exists t0. split; auto. }
-      { apply IHs in inImage. destruct inImage; auto. } } }
-  destruct GenLemma.
+    { destruct a. simpl in IN_IMAGE. simpl. destruct (Nat.eq_dec n x).
+      { inversion IN_IMAGE. subst. apply apply_subst_FV in IN_FV.
+        destruct IN_FV; auto. left. exists t0. split; auto. }
+      { apply IHs in IN_IMAGE. destruct IN_IMAGE; auto. } } }
+  destruct GEN.
   { left. red. eauto. }
   { right. auto. }
 Qed.
@@ -254,206 +255,233 @@ Definition more_general (m s : subst) : Prop :=
 (* Unification property *)
 Definition unifier (s : subst) (t1 t2 : term) : Prop := apply_subst s t1 = apply_subst s t2.
 
-(* MGU *)
-(* Definition mgu (m : subst) (t1 t2 : term) : Prop :=
-  unifier m t1 t2 /\ forall (s : subst), unifier s t1 t2 -> more_general m s.
-*)
-
 Inductive unification_step_outcome : Set :=
-| Fail : unification_step_outcome
-| Fine : unification_step_outcome
-| Subst : forall (n: name) (t: term), unification_step_outcome.
+| NonUnifiable : unification_step_outcome
+| Same : unification_step_outcome
+| VarSubst : forall (n: name) (t: term), unification_step_outcome.
 
 Definition create (n: name) (t: term) : unification_step_outcome :=
-  if occurs n t then Fail else Subst n t.
+  if occurs n t then NonUnifiable else VarSubst n t.
+
+Lemma inv_create
+      (n0 n1 : name)
+      (t0 t1 : term)
+      (CR : create n0 t0 = VarSubst n1 t1) :
+      t0 = t1.
+Proof.
+  { intros. unfold create in CR. destruct (occurs n0 t0).
+    { inversion CR. }
+    { inversion CR. reflexivity. } }
+Qed.
 
 (* Find a difference in a couple of terms and try to make a unification step *)
 Fixpoint unification_step (t1 t2 : term) : unification_step_outcome :=
   match (t1, t2) with
-  | (Cst n1      , Cst n2      ) => if eq_nat_dec n1 n2 then Fine else Fail 
+  | (Cst n1      , Cst n2      ) => if eq_nat_dec n1 n2 then Same else NonUnifiable 
   | (Con n1 l1 r1, Con n2 l2 r2) => if eq_nat_dec n1 n2
                                     then
                                       match unification_step l1 l2 with
-                                      | Fail => Fail
-                                      | Fine => unification_step r1 r2
+                                      | NonUnifiable => NonUnifiable
+                                      | Same => unification_step r1 r2
                                       | res  => res
                                       end
-                                    else Fail
-  | (Var n1      , Var n2      ) => if eq_nat_dec n1 n2 then Fine else create n1 t2
+                                    else NonUnifiable
+  | (Var n1      , Var n2      ) => if eq_nat_dec n1 n2 then Same else create n1 t2
   | (Var n1      , _           ) => create n1 t2
   | (_           , Var n2      ) => create n2 t1
-  | (_           , _           ) => Fail
+  | (_           , _           ) => NonUnifiable
   end.
 
-Definition unification_step_ok t1 t2 n s := unification_step t1 t2 = Subst n s.
+Definition unification_step_ok t1 t2 n s := unification_step t1 t2 = VarSubst n s.
 
-Lemma unification_step_fv: forall t1 t2 s n ,
-    unification_step_ok t1 t2 n s -> (forall m, In m (fv_term s) -> In m (fv_term t1) \/ In m (fv_term t2)).
+Lemma unification_step_fv
+     (t1 t2 s : term)
+     (n m : name)
+     (STEP_OK : unification_step_ok t1 t2 n s)
+     (M_FV : In m (fv_term s)) :
+     In m (fv_term t1) \/ In m (fv_term t2).
 Proof.
-  assert (invCr: forall n0 n1 t0 t1, create n0 t0 = Subst n1 t1 -> t0 = t1).
-  { intros. unfold create in H. destruct (occurs n0 t0).
-    - inversion H.
-    - inversion H. reflexivity. }
-  induction t1.
-  * intros. unfold unification_step_ok in H. destruct t2; unfold unification_step in H.
-    + destruct (Nat.eq_dec n n1).
-      - inversion H.
-      - apply invCr in H; subst. right. assumption.
-    + apply invCr in H; subst. right. assumption.
-    + apply invCr in H; subst. right. assumption.
-  * intros. unfold unification_step_ok in H. destruct t2; unfold unification_step in H.
-    + apply invCr in H; subst. left. assumption.
-    + destruct (Nat.eq_dec n n1); inversion H.
-    + inversion H.
-  * intros. unfold unification_step_ok in H. destruct t2; unfold unification_step in H.
-    + apply invCr in H; subst. left. assumption.
-    + inversion H.
-    + fold unification_step in H. destruct (Nat.eq_dec n n1).
-      - destruct (unification_step t1_1 t2_1) eqn:eq.
-        { inversion H. }
-        { unfold unification_step_ok in IHt1_2. apply IHt1_2 with (m := m) in H.
-          - destruct H.
-            + left. unfold fv_term. fold fv_term. apply (set_union_intro name_eq_dec). right. assumption.
-            + right. unfold fv_term. fold fv_term. apply (set_union_intro name_eq_dec). right. assumption.
-          - assumption. }
-        { inversion H; subst. unfold unification_step_ok in IHt1_1.
+  revert M_FV STEP_OK. revert t2 m n. induction t1.
+  { intros. unfold unification_step_ok in STEP_OK.
+    destruct t2; unfold unification_step in STEP_OK.
+    { destruct (Nat.eq_dec n n1).
+      { inversion STEP_OK. }
+      { apply inv_create in STEP_OK; subst. right. assumption. } }
+    { apply inv_create in STEP_OK; subst. right. assumption. }
+    { apply inv_create in STEP_OK; subst. right. assumption. } }
+  { intros. unfold unification_step_ok in STEP_OK.
+    destruct t2; unfold unification_step in STEP_OK.
+    { apply inv_create in STEP_OK; subst. left. assumption. }
+    { destruct (Nat.eq_dec n n1); inversion STEP_OK. }
+    { inversion STEP_OK. } }
+  { intros. unfold unification_step_ok in STEP_OK.
+    destruct t2; unfold unification_step in STEP_OK.
+    { apply inv_create in STEP_OK; subst. left. assumption. }
+    { inversion STEP_OK. }
+    { fold unification_step in STEP_OK. destruct (Nat.eq_dec n n1).
+      { destruct (unification_step t1_1 t2_1) eqn:eq.
+        { inversion STEP_OK. }
+        { unfold unification_step_ok in IHt1_2. apply IHt1_2 with (m := m) in STEP_OK.
+          { destruct STEP_OK.
+            { left. unfold fv_term. fold fv_term. apply (set_union_intro name_eq_dec). right. assumption. }
+            { right. unfold fv_term. fold fv_term. apply (set_union_intro name_eq_dec). right. assumption. } }
+          { assumption. } }
+        { inversion STEP_OK; subst. unfold unification_step_ok in IHt1_1.
           apply IHt1_1 with (m := m) in eq.
-          - destruct eq.
-            + left. unfold fv_term. fold fv_term. apply (set_union_intro name_eq_dec). left. assumption.
-            + right. unfold fv_term. fold fv_term. apply (set_union_intro name_eq_dec). left. assumption.
-          - assumption. }
-      - inversion H.
+          { destruct eq.
+            { left. unfold fv_term. fold fv_term. apply (set_union_intro name_eq_dec). left. assumption. }
+            { right. unfold fv_term. fold fv_term. apply (set_union_intro name_eq_dec). left. assumption. } }
+          { assumption. } } }
+      { inversion STEP_OK. } } }
 Qed.
 
-Lemma unification_step_subst_wf:
-  forall t1 t2 s n, unification_step_ok t1 t2 n s -> ~ In n (fv_term s).
+Lemma unification_step_subst_wf
+      (t1 t2 s : term)
+      (n : name)
+      (STEP_OK : unification_step_ok t1 t2 n s) :
+      ~ In n (fv_term s).
 Proof.
-  intros. assert (exists m t, create m t = Subst n s).
-  {
-    generalize dependent t2. induction t1; intros.
-    * destruct t2; unfold unification_step_ok in H; unfold unification_step in H.
-      + destruct (Nat.eq_dec n0 n1).
-         - inversion H.
-         - eexists. eexists. eapply H.
-      + eexists. eexists. eapply H.
-      + eexists. eexists. eapply H.
-    * destruct t2; unfold unification_step_ok in H; unfold unification_step in H.
-      + eexists. eexists. eapply H.
-      + destruct (Nat.eq_dec n0 n1); inversion H.
-      + inversion H.
-    * destruct t2; unfold unification_step_ok in H; unfold unification_step in H.
-      + eexists. eexists. eapply H.
-      + inversion H.
-      + destruct (Nat.eq_dec n0 n1).
-        - fold unification_step in H. destruct (unification_step t1_1 t2_1) eqn:eq.
-          { inversion H. }
-          { eapply IHt1_2. unfold unification_step_ok. eapply H. }
-          { inversion H; subst. eapply IHt1_1. unfold unification_step_ok.
-            eapply eq. }
-        - inversion H.
-  }
-  destruct H0. destruct H0. unfold create in H0. destruct (occurs x x0) eqn:eq.
-  - inversion H0.
-  - inversion H0; subst. intros CH. apply occurs_In in CH. rewrite eq in CH.
-    inversion CH.
+  intros. assert (CR : exists m t, create m t = VarSubst n s).
+  { revert STEP_OK. revert t2. induction t1; intros.
+    { destruct t2; unfold unification_step_ok in STEP_OK; unfold unification_step in STEP_OK.
+      { destruct (Nat.eq_dec n0 n1).
+        { inversion STEP_OK. }
+        { eexists. eexists. eapply STEP_OK. } }
+      { eexists. eexists. eapply STEP_OK. }
+      { eexists. eexists. eapply STEP_OK. } }
+    { destruct t2; unfold unification_step_ok in STEP_OK; unfold unification_step in STEP_OK.
+      { eexists. eexists. eapply STEP_OK. }
+      { destruct (Nat.eq_dec n0 n1); inversion STEP_OK. }
+      { inversion STEP_OK. } }
+    { destruct t2; unfold unification_step_ok in STEP_OK; unfold unification_step in STEP_OK.
+      { eexists. eexists. eapply STEP_OK. }
+      { inversion STEP_OK. }
+      { destruct (Nat.eq_dec n0 n1).
+        { fold unification_step in STEP_OK. destruct (unification_step t1_1 t2_1) eqn:eq.
+          { inversion STEP_OK. }
+          { eapply IHt1_2. unfold unification_step_ok. eapply STEP_OK. }
+          { inversion STEP_OK; subst. eapply IHt1_1. unfold unification_step_ok.
+            eapply eq. } }
+        { inversion STEP_OK. } } } }
+  destruct CR as [m [t CR]]. unfold create in CR. destruct (occurs m t) eqn:eq.
+  { inversion CR. }
+  { good_inversion CR. intros CH. apply occurs_In in CH. rewrite eq in CH.
+    inversion CH. }
 Qed.
 
-Lemma unification_step_subst_occurs:
-  forall t1 t2 s n, unification_step_ok t1 t2 n s -> In n (fv_term t1) \/ In n (fv_term t2).
+Lemma unification_step_subst_occurs
+      (t1 t2 s : term)
+      (n : name)
+      (STEP_OK : unification_step_ok t1 t2 n s) :
+      In n (fv_term t1) \/ In n (fv_term t2).
 Proof.
-  assert (invCr: forall n0 n1 t0 t1, create n0 t0 = Subst n1 t1 -> n0 = n1).
+  assert (INV_CR: forall n0 n1 t0 t1, create n0 t0 = VarSubst n1 t1 -> n0 = n1).
   { intros. unfold create in H. destruct (occurs n0 t0).
-    - inversion H.
-    - inversion H. reflexivity. }
-  assert (fvInFv: forall n, In n (fv_term (Var n))).
+    { inversion H. }
+    { inversion H. reflexivity. } }
+  assert (VAR_IN_FV: forall n, In n (fv_term (Var n))).
   { unfold fv_term. unfold In. left. reflexivity. }
-  induction t1.
-  * intros. unfold unification_step_ok in H. destruct t2; unfold unification_step in H.
-    + destruct (Nat.eq_dec n n1).
-      - inversion H.
-      - apply invCr in H; subst. left. apply fvInFv.
-    + apply invCr in H; subst. left. apply fvInFv.
-    + apply invCr in H; subst. left. apply fvInFv.
-  * intros. unfold unification_step_ok in H. destruct t2; unfold unification_step in H.
-    + apply invCr in H; subst. right. apply fvInFv.
-    + destruct (Nat.eq_dec n n1); inversion H.
-    + inversion H.
-  * intros. unfold unification_step_ok in H. destruct t2; unfold unification_step in H.
-    + apply invCr in H; subst. right. apply fvInFv.
-    + inversion H.
-    + fold unification_step in H. destruct (unification_step t1_1 t2_1) eqn:eq.
-      - destruct (Nat.eq_dec n n1); inversion H.
-      - destruct (Nat.eq_dec n n1).
-        { unfold unification_step_ok in IHt1_2. apply IHt1_2 in H. destruct H.
-          * left. unfold fv_term. fold fv_term. apply (set_union_intro name_eq_dec). right. assumption.
-          * right. unfold fv_term. fold fv_term. apply (set_union_intro name_eq_dec). right. assumption. }
-        inversion H.
-      - destruct (Nat.eq_dec n n1); inversion H; subst.
+  revert STEP_OK. revert n t2. induction t1.
+  { intros. unfold unification_step_ok in STEP_OK.
+    destruct t2; unfold unification_step in STEP_OK.
+    { destruct (Nat.eq_dec n n1).
+      { inversion STEP_OK. }
+      { apply INV_CR in STEP_OK; subst. left. apply VAR_IN_FV. } }
+    { apply INV_CR in STEP_OK; subst. left. apply VAR_IN_FV. }
+    { apply INV_CR in STEP_OK; subst. left. apply VAR_IN_FV. } }
+  { intros. unfold unification_step_ok in STEP_OK. destruct t2; unfold unification_step in STEP_OK.
+    { apply INV_CR in STEP_OK; subst. right. apply VAR_IN_FV. }
+    { destruct (Nat.eq_dec n n1); inversion STEP_OK. }
+    { inversion STEP_OK. } }
+  { intros. unfold unification_step_ok in STEP_OK. destruct t2; unfold unification_step in STEP_OK.
+    { apply INV_CR in STEP_OK; subst. right. apply VAR_IN_FV. }
+    { inversion STEP_OK. }
+    { fold unification_step in STEP_OK. destruct (unification_step t1_1 t2_1) eqn:eq.
+      { destruct (Nat.eq_dec n n1); inversion STEP_OK. }
+      { destruct (Nat.eq_dec n n1).
+        { unfold unification_step_ok in IHt1_2. apply IHt1_2 in STEP_OK. destruct STEP_OK.
+          { left. unfold fv_term. fold fv_term. apply (set_union_intro name_eq_dec). right. assumption. }
+          { right. unfold fv_term. fold fv_term. apply (set_union_intro name_eq_dec). right. assumption. } }
+        { inversion STEP_OK. } }
+      { destruct (Nat.eq_dec n n1); inversion STEP_OK; subst.
         unfold unification_step_ok in IHt1_1. apply IHt1_1 in eq. destruct eq.
         { left. unfold fv_term. fold fv_term. apply (set_union_intro name_eq_dec). left. assumption. }
-        right. unfold fv_term. fold fv_term. apply (set_union_intro name_eq_dec). left. assumption.
+        { right. unfold fv_term. fold fv_term. apply (set_union_intro name_eq_dec). left. assumption. } } } }
 Qed.
 
-Lemma unification_step_subst_elims: forall s t n, In n (fv_term (apply_subst (singleton_subst n s) t)) -> In n (fv_term s).
+Lemma unification_step_subst_elims
+      (s t : term)
+      (n : name)
+      (N_FV : In n (fv_term (apply_subst (singleton_subst n s) t))) :
+      In n (fv_term s).
 Proof.
-  intros s t n. unfold singleton_subst. induction t.
-  * unfold apply_subst. unfold image. destruct (Nat.eq_dec n n0).
-    + auto.
-    + unfold fv_term. intros. exfalso. inversion H.
-      - apply n1. symmetry. assumption.
-      - inversion H0.
-  * intros. inversion H.
-  * intros. unfold apply_subst in H. fold apply_subst in H. unfold fv_term in H. fold fv_term in H.
-    apply (set_union_elim name_eq_dec) in H. destruct H; auto.
+  revert N_FV. unfold singleton_subst. induction t.
+  { unfold apply_subst. unfold image. destruct (Nat.eq_dec n n0).
+    { auto. }
+    { unfold fv_term. intros. exfalso. inversion N_FV.
+      { apply n1. symmetry. assumption. }
+      { inversion H. } } }
+  { intros. inversion N_FV. }
+  { intros. unfold apply_subst in N_FV. fold apply_subst in N_FV.
+    unfold fv_term in N_FV. fold fv_term in N_FV.
+    apply (set_union_elim name_eq_dec) in N_FV. destruct N_FV; auto. }
 Qed.
 
-Lemma lt_size:
-  forall (vs1 vs2 : var_set),
-    NoDup vs1 -> NoDup vs2 -> incl vs1 vs2 -> (exists n, In n vs2 /\ ~ (In n vs1)) -> var_set_size vs1 < var_set_size vs2.
+Lemma lt_size
+      (vs1 vs2 : var_set)
+      (NO_DUP_1 : NoDup vs1)
+      (NO_DUP_2 : NoDup vs2)
+      (INCL : incl vs1 vs2)
+      (UNIQ_VAR : exists n, In n vs2 /\ ~ (In n vs1)) :
+      var_set_size vs1 < var_set_size vs2.
 Proof.
-  intros. destruct H2. destruct H2. apply in_split in H2.
-  destruct H2. destruct H2. subst.
+  intros. destruct UNIQ_VAR as [n [IN NOT_IN]].
+  apply in_split in IN.
+  destruct IN as [l1 [l2 EQ]]. subst.
   unfold var_set_size. rewrite app_length. simpl.
-  assert (length vs1 <= length (x0 ++ x1)).
+  assert (LE_LEN : length vs1 <= length (l1 ++ l2)).
   { apply NoDup_incl_length.
-    * assumption.
-    * unfold incl. intros. assert (H2_copy := H2).
-      apply H1 in H2. apply in_app_or in H2. destruct H2.
-      + apply in_or_app. left. assumption.
-      + inversion H2.
-        - exfalso. apply H3. congruence.
-        - apply in_or_app. right. assumption. }
-  rewrite app_length in H2. omega.
+    { assumption. }
+    { unfold incl. intros. assert (H_COPY := H).
+      apply INCL in H. apply in_app_or in H. destruct H.
+      { apply in_or_app. left. auto. }
+      { inversion H.
+        { exfalso. subst. auto. }
+        { apply in_or_app. right. auto. } } } }
+  rewrite app_length in LE_LEN. omega.
 Qed.
 
-Lemma unification_step_decreases_fv:
-  forall t1 t2 s n,
-    unification_step_ok t1 t2 n s ->
-    var_set_size (var_set_union (fv_term (apply_subst (singleton_subst n s) t1)) (fv_term (apply_subst [(n, s)] t2))) < var_set_size (var_set_union (fv_term t1) (fv_term t2)).
+Lemma unification_step_decreases_fv
+      (t1 t2 s : term)
+      (n : name)
+      (STEP_OK : unification_step_ok t1 t2 n s) :
+      var_set_size (var_set_union (fv_term (apply_subst (singleton_subst n s) t1)) (fv_term (apply_subst (singleton_subst n s) t2))) <
+      var_set_size (var_set_union (fv_term t1) (fv_term t2)).
 Proof.
-  intros t1 t2 s n USok.
   apply lt_size; try apply union_NoDup.
-  * apply set_union_nodup; apply fv_term_nodup.
-  * apply set_union_nodup; apply fv_term_nodup.
-  * intros n0 InH. apply (set_union_elim name_eq_dec) in InH. inversion_clear InH.
-    + apply apply_subst_FV in H. inversion_clear H.
-      - apply (set_union_intro name_eq_dec). left. assumption.
-      - apply unification_step_fv with (m:=n0) in USok.
+  { apply set_union_nodup; apply fv_term_nodup. }
+  { apply set_union_nodup; apply fv_term_nodup. }
+  { intros n0 InH. apply (set_union_elim name_eq_dec) in InH. inversion_clear InH.
+    { apply apply_subst_FV in H. inversion_clear H.
+      { apply (set_union_intro name_eq_dec). left. assumption. }
+      { apply unification_step_fv with (m:=n0) in STEP_OK.
         { apply (set_union_intro name_eq_dec). assumption. }
         red in H0. destruct H0 as [x [t [xImage inFV]]]. simpl in xImage.
-        destruct (Nat.eq_dec n x); good_inversion xImage. auto.
-    + apply apply_subst_FV in H. inversion_clear H.
-      - apply (set_union_intro name_eq_dec). right. assumption.
-      - apply unification_step_fv with (m:=n0) in USok.
+        destruct (Nat.eq_dec n x); good_inversion xImage. auto. } }
+    { apply apply_subst_FV in H. inversion_clear H.
+      { apply (set_union_intro name_eq_dec). right. assumption. }
+      { apply unification_step_fv with (m:=n0) in STEP_OK.
         { apply (set_union_intro name_eq_dec). assumption. }
         red in H0. destruct H0 as [x [t [xImage inFV]]]. simpl in xImage.
-        destruct (Nat.eq_dec n x); good_inversion xImage. auto.
-  * exists n. split.
-    + apply unification_step_subst_occurs in USok. apply (set_union_intro name_eq_dec). assumption.
-    + unfold not. intro H. apply (set_union_elim name_eq_dec) in H. inversion_clear H as [H0 | H0];
+        destruct (Nat.eq_dec n x); good_inversion xImage. auto. } } }
+  { exists n. split.
+    { apply unification_step_subst_occurs in STEP_OK. apply (set_union_intro name_eq_dec). assumption. }
+    { unfold not. intro H. apply (set_union_elim name_eq_dec) in H. inversion_clear H as [H0 | H0];
       apply unification_step_subst_elims in H0;
-      apply unification_step_subst_wf in USok; auto.
+      apply unification_step_subst_wf in STEP_OK; auto. } }
 Qed.
+
+
 
 Definition terms := (term * term)%type.
 
@@ -461,271 +489,314 @@ Definition fvOrder (t : terms) := length (var_set_union (fv_term (fst t)) (fv_te
 
 Definition fvOrderRel (t p : terms) := fvOrder t < fvOrder p.
 
-Hint Constructors Acc.
+(* Hint Constructors Acc. *)
 
-Theorem fvOrder_wf: well_founded fvOrderRel.
+Theorem fvOrder_wf : well_founded fvOrderRel.
 Proof.
   assert (fvOrder_wf': forall (size: nat) (t: terms), fvOrder t < size -> Acc fvOrderRel t).
-    {unfold fvOrderRel. induction size.
-     * intros. inversion H.
-     * intros. constructor. intros. apply IHsize. omega.
-    }
+  { unfold fvOrderRel. induction size.
+    { intros. inversion H. }
+    { intros. constructor. intros. apply IHsize. omega. } }
   red; intro; eapply fvOrder_wf'; eauto.
 Defined.
 
-Inductive unify : term -> term -> option subst -> Set :=
-| unify_Fail : forall t1 t2, unification_step t1 t2 = Fail -> unify t1 t2 None
-| unify_Fine : forall t1 t2, unification_step t1 t2 = Fine -> unify t1 t2 (Some empty_subst)
-| unify_SubstNone : forall t1 t2 n s, unification_step t1 t2 = Subst n s ->
-                                      unify (apply_subst (singleton_subst n s) t1) (apply_subst (singleton_subst n s) t2) None ->
-                                      unify t1 t2 None
-| unify_SubstSome : forall t1 t2 n s r sr, unification_step t1 t2 = Subst n s ->
-                                           unify (apply_subst (singleton_subst n s) t1) (apply_subst (singleton_subst n s) t2) (Some r) ->
-                                           sr = compose (singleton_subst n s) r ->
-                                           unify t1 t2 (Some sr).
+Inductive mgu : term -> term -> option subst -> Set :=
+| mguNonUnifiable : forall t1 t2 (STEP_NU : unification_step t1 t2 = NonUnifiable),
+                                 mgu t1 t2 None
+| mguSame :         forall t1 t2 (STEP_SAME : unification_step t1 t2 = Same),
+                                 mgu t1 t2 (Some empty_subst)
+| mguVarSubstNone : forall t1 t2 n s
+                           (STEP_SUBST : unification_step t1 t2 = VarSubst n s)
+                           (THEN_FAIL : mgu (apply_subst (singleton_subst n s) t1) (apply_subst (singleton_subst n s) t2) None),
+                           mgu t1 t2 None
+| mguVarSubstSome : forall t1 t2 n s r sr
+                           (STEP_SUBST : unification_step t1 t2 = VarSubst n s)
+                           (THEN_SUCC : mgu (apply_subst (singleton_subst n s) t1) (apply_subst (singleton_subst n s) t2) (Some r))
+                           (SR_EQ : sr = compose (singleton_subst n s) r),
+                           mgu t1 t2 (Some sr).
 
-Example test1: unify (Cst 1)                 (Cst 2)                 None.                            Proof. repeat econstructor. Qed.
-Example test2: unify (Cst 1)                 (Cst 1)                 (Some []).                       Proof. repeat econstructor. Qed.
-Example test3: unify (Var 1)                 (Var 2)                 (Some [(1, Var 2)]).             Proof. repeat econstructor. Qed.
-Example test4: unify (Var 1)                 (Var 1)                 (Some []).                       Proof. repeat econstructor. Qed.
-Example test5: unify (Con 1 (Var 1) (Var 2)) (Con 2 (Var 1) (Var 2)) None.                            Proof. repeat econstructor. Qed.
-Example test6: unify (Con 1 (Var 1) (Var 2)) (Con 1 (Var 1) (Var 2)) (Some []).                       Proof. repeat econstructor. Qed.
-Example test7: unify (Con 1 (Var 1) (Var 1)) (Con 1 (Var 1) (Var 2)) (Some [(1, Var 2)]).             Proof. repeat econstructor. Qed.
-Example test8: unify (Con 1 (Cst 1) (Var 2)) (Con 1 (Var 1) (Cst 2)) (Some [(1, Cst 1); (2, Cst 2)]). Proof. econstructor. econstructor. eapply unify_SubstSome. econstructor. econstructor. econstructor. econstructor. econstructor. Qed.
+Example test1: mgu (Cst 1) (Cst 2) None.
+Proof. repeat econstructor. Qed.
 
-Lemma unify_exists : forall t1 t2, {r & unify t1 t2 r}.
+Example test2: mgu (Cst 1) (Cst 1) (Some []).
+Proof. repeat econstructor. Qed.
+
+Example test3: mgu (Var 1) (Var 2) (Some [(1, Var 2)]).
+Proof. repeat econstructor. Qed.
+
+Example test4: mgu (Var 1) (Var 1) (Some []).
+Proof. repeat econstructor. Qed.
+
+Example test5: mgu (Con 1 (Var 1) (Var 2)) (Con 2 (Var 1) (Var 2)) None.
+Proof. repeat econstructor. Qed.
+
+Example test6: mgu (Con 1 (Var 1) (Var 2)) (Con 1 (Var 1) (Var 2)) (Some []).
+Proof. repeat econstructor. Qed.
+
+Example test7: mgu (Con 1 (Var 1) (Var 1)) (Con 1 (Var 1) (Var 2)) (Some [(1, Var 2)]).
+Proof. repeat econstructor. Qed.
+
+Example test8: mgu (Con 1 (Cst 1) (Var 2)) (Con 1 (Var 1) (Cst 2)) (Some [(1, Cst 1); (2, Cst 2)]).
 Proof.
-  intros t1 t2.
-  remember (fun p => {r : option subst & unify (fst p) (snd p) r}) as P.
+  econstructor.
+  1, 3: econstructor.
+  repeat econstructor.
+Qed.
+
+
+
+Lemma mgu_exists
+      (t1 t2 : term) :
+      {r & mgu t1 t2 r}.
+Proof.
+  remember (fun p => {r : option subst & mgu (fst p) (snd p) r}) as P.
   assert (P (t1, t2)).
-  {
-    apply well_founded_induction with (R := fvOrderRel).
-    * apply fvOrder_wf.
-    * intros. subst. clear t1 t2. destruct x as [t1 t2]. simpl.
+  { apply well_founded_induction with (R := fvOrderRel).
+    { apply fvOrder_wf. }
+    { intros. subst. clear t1 t2. destruct x as [t1 t2]. simpl.
       destruct (unification_step t1 t2) eqn:eq.
-      + exists None. constructor. assumption.
-      + exists (Some empty_subst). constructor. assumption.
-      + specialize (H (apply_subst (singleton_subst n t) t1, apply_subst (singleton_subst n t) t2)).
+      { exists None. constructor. assumption. }
+      { exists (Some empty_subst). constructor. assumption. }
+      { specialize (H (apply_subst (singleton_subst n t) t1, apply_subst (singleton_subst n t) t2)).
         assert (fvOr : fvOrderRel (apply_subst (singleton_subst n t) t1, apply_subst (singleton_subst n t) t2) (t1, t2)).
         { apply unification_step_decreases_fv. assumption. }
         specialize (H fvOr). destruct H. destruct x.
-        - eexists. eapply unify_SubstSome.
+        { eexists. eapply mguVarSubstSome.
           { eassumption. }
           { eassumption. }
-          { reflexivity. }
-        - exists None. eapply unify_SubstNone.
+          { reflexivity. } }
+        { exists None. eapply mguVarSubstNone.
           { eassumption. }
-          { eassumption. }
-  }
+          { eassumption. } } } } }
   subst. assumption.
 Qed.
 
-Lemma unify_unique : forall t1 t2 r r', unify t1 t2 r -> unify t1 t2 r' -> r = r'.
+Lemma mgu_unique
+      (t1 t2 : term)
+      (r r' : option subst)
+      (UNI_1 : mgu t1 t2 r)
+      (UNI_2 : mgu t1 t2 r') :
+      r = r'.
 Proof.
-  intros t1 t2 r r' H. revert r'. induction H.
-  * intros. inversion H; try reflexivity; rewrite e in H0; inversion H0.
-  * intros. inversion H; try reflexivity; rewrite e in H0; inversion H0.
-  * intros. inversion H0; try reflexivity.
-    + rewrite e in H1; inversion H1.
-    + rewrite e in H1; inversion H1. subst. apply IHunify in H2. inversion H2.
-  * intros. inversion H0.
-    + rewrite e in H1. inversion H1.
-    + rewrite e in H1. inversion H1.
-    + rewrite e in H1. inversion H1. subst.
-      apply IHunify in H2. inversion H2.
-    + rewrite e in H1. inversion H1. subst.
-      apply IHunify in H2. inversion H2. reflexivity.
+  revert UNI_2. revert r'. induction UNI_1.
+  { intros. good_inversion UNI_2; try reflexivity; congruence. }
+  { intros. good_inversion UNI_2; try reflexivity; congruence. }
+  { intros. good_inversion UNI_2; try reflexivity; try congruence.
+    rewrite STEP_SUBST0 in STEP_SUBST. good_inversion STEP_SUBST.
+    apply IHUNI_1 in THEN_SUCC. inversion THEN_SUCC. }
+  { intros. good_inversion UNI_2; try congruence;
+    rewrite STEP_SUBST0 in STEP_SUBST; good_inversion STEP_SUBST.
+    { apply IHUNI_1 in THEN_FAIL; inversion THEN_FAIL. }
+    { apply IHUNI_1 in THEN_SUCC; inversion THEN_SUCC; auto. } }
 Qed.
 
-Lemma fine_step_equal_terms :
-  forall t1 t2,
-    unification_step t1 t2 = Fine -> t1 = t2.
+Lemma same_step_equal_terms
+      (t1 t2 : term)
+      (STEP_SAME : unification_step t1 t2 = Same) :
+      t1 = t2.
 Proof.
-  assert (createFine : forall n t, create n t <> Fine).
+  assert (CREATE_NOT_SAME : forall n t, create n t <> Same).
   { unfold create. intros n t C. destruct (occurs n t); inversion C. }
-  induction t1; induction t2; intro us_eq; inversion us_eq; clear us_eq; subst.
-  - destruct (Nat.eq_dec n n0).
+  revert STEP_SAME. revert t2. induction t1; induction t2; intros; good_inversion STEP_SAME.
+  { destruct (Nat.eq_dec n n0).
     { congruence. }
-    { apply createFine in H0. contradiction. }
-  - apply createFine in H0. contradiction.
-  - destruct (Nat.eq_dec n n0).
+    { apply CREATE_NOT_SAME in H0. contradiction. } }
+  { apply CREATE_NOT_SAME in H0. contradiction. }
+  { destruct (Nat.eq_dec n n0).
     { congruence. }
-    { inversion H0. }
-  - apply createFine in H0. contradiction.
-  - destruct (Nat.eq_dec n n0).
+    { inversion H0. } }
+  { apply CREATE_NOT_SAME in H0. contradiction. }
+  { destruct (Nat.eq_dec n n0).
     { subst. destruct (unification_step t1_1 t2_1) eqn:eq; inversion H0.
       apply IHt1_1 in eq. apply IHt1_2 in H0. congruence. }
-    { inversion H0. }
+    { inversion H0. } }
 Qed.
 
-
-Lemma unify_unifies:
-  forall t1 t2 s,
-    unify t1 t2 (Some s) -> unifier s t1 t2.
+Lemma mgu_unifies
+      (t1 t2 : term)
+      (s : subst)
+      (UNI : mgu t1 t2 (Some s)) :
+      unifier s t1 t2.
 Proof.
-  intros t1 t2. remember (fun p => forall s : subst,
-      unify (fst p) (snd p) (Some s) -> unifier s (fst p) (snd p)).
+  revert UNI. revert s.
+  remember (fun p => forall s : subst,
+      mgu (fst p) (snd p) (Some s) -> unifier s (fst p) (snd p)).
   assert (P (t1, t2)).
-  {
-    apply well_founded_induction with (R := fvOrderRel).
-    * apply fvOrder_wf.
-    * intros. subst. clear t1 t2. destruct x as [t1 t2]. simpl.
+  { apply well_founded_induction with (R := fvOrderRel).
+    { apply fvOrder_wf. }
+    { intros. subst. clear t1 t2. destruct x as [t1 t2]. simpl.
       intros. inversion H0; subst; clear H0.
-      + unfold unifier. rewrite apply_empty. rewrite apply_empty.
-        apply fine_step_equal_terms. assumption.
-      + assert (fvOr : fvOrderRel (apply_subst (singleton_subst n s0) t1, apply_subst (singleton_subst n s0) t2) (t1, t2)).
+      { unfold unifier. rewrite apply_empty. rewrite apply_empty.
+        apply same_step_equal_terms. assumption. }
+      { assert (fvOr : fvOrderRel (apply_subst (singleton_subst n s0) t1, apply_subst (singleton_subst n s0) t2) (t1, t2)).
         { apply unification_step_decreases_fv. assumption. }
         eapply H in fvOr.
         2: { eassumption. }
         { unfold unifier. rewrite compose_correctness. rewrite compose_correctness.
-          assumption. }
-  }
+          assumption. } } } }
   subst. assumption.
 Qed.
 
-Lemma unification_step_binds :
-  forall t1 t2 x t s,
-    unification_step t1 t2 = Subst x t ->
-    unifier s t1 t2 ->
-    apply_subst s (Var x) = apply_subst s t.
+Lemma unification_step_binds
+      (t1 t2 t : term)
+      (x : name)
+      (s : subst)
+      (STEP : unification_step t1 t2 = VarSubst x t)
+      (S_UNIFIER : unifier s t1 t2) :
+      apply_subst s (Var x) = apply_subst s t.
 Proof.
-  induction t1; induction t2; intros; simpl in H.
-  * destruct (Nat.eq_dec n n0).
-    + inversion H.
-    + unfold create in H. destruct (occurs n (Var n0)); inversion H.
-      subst. assumption.
-  * unfold create in H. destruct (occurs n (Cst n0)); inversion H. subst. assumption.
-  * unfold create in H. destruct (occurs n (Con n0 t2_1 t2_2)); inversion H. subst. assumption.
-  * unfold create in H. destruct (occurs n0 (Cst n)); inversion H. subst. symmetry. assumption.
-  * destruct (Nat.eq_dec n n0); inversion H.
-  * inversion H.
-  * unfold create in H. destruct (occurs n0 (Con n t1_1 t1_2)); inversion H. subst. symmetry. assumption.
-  * inversion H.
-  * clear IHt2_1. clear IHt2_2.
+  revert S_UNIFIER STEP. revert s x t t2.
+  induction t1; induction t2; intros; simpl in STEP.
+  { destruct (Nat.eq_dec n n0).
+    { inversion STEP. }
+    { unfold create in STEP. destruct (occurs n (Var n0)); inversion STEP.
+      subst. assumption. } }
+  { unfold create in STEP. destruct (occurs n (Cst n0)); inversion STEP. subst. assumption. }
+  { unfold create in STEP. destruct (occurs n (Con n0 t2_1 t2_2)); inversion STEP. subst. assumption. }
+  { unfold create in STEP. destruct (occurs n0 (Cst n)); inversion STEP. subst. symmetry. assumption. }
+  { destruct (Nat.eq_dec n n0); inversion STEP. }
+  { inversion STEP. }
+  { unfold create in STEP. destruct (occurs n0 (Con n t1_1 t1_2)); inversion STEP. subst. symmetry. assumption. }
+  { inversion STEP. }
+  { clear IHt2_1. clear IHt2_2.
     destruct (Nat.eq_dec n n0).
-    + subst. destruct (unification_step t1_1 t2_1) eqn:eq.
-      - inversion H.
-      - inversion H0. apply IHt1_2 with t2_2; assumption.
-      - inversion H. subst. inversion H0. apply IHt1_1 with t2_1; assumption.
-    + inversion H.
+    { subst. destruct (unification_step t1_1 t2_1) eqn:eq.
+      { inversion STEP. }
+      { inversion S_UNIFIER. apply IHt1_2 with t2_2; assumption. }
+      { inversion STEP. subst. inversion S_UNIFIER. apply IHt1_1 with t2_1; assumption. } }
+    { inversion STEP. } }
 Qed.
 
-Lemma unification_step_binds_2 :
-  forall t1 t2 x t s,
-    unification_step t1 t2 = Subst x t ->
-    unifier s t1 t2 ->
-    forall t', apply_subst s t' = apply_subst s (apply_subst (singleton_subst x t) t').
+Lemma unification_step_binds_2
+      (t1 t2 t : term)
+      (x : name)
+      (s : subst)
+      (STEP : unification_step t1 t2 = VarSubst x t)
+      (S_UNIFIER : unifier s t1 t2)
+      (t' : term) :
+      apply_subst s t' = apply_subst s (apply_subst (singleton_subst x t) t').
 Proof.
-  intros. specialize (unification_step_binds t1 t2 x t s H H0). intro.
+  specialize (unification_step_binds _ _ _ _ _ STEP S_UNIFIER). intro APP_EQ.
   induction t'.
-  * simpl. destruct (Nat.eq_dec x n).
-    + subst. rewrite <- H1. reflexivity.
-    + reflexivity.
-  * reflexivity.
-  * simpl. rewrite IHt'1. rewrite IHt'2. reflexivity.
+  { simpl. destruct (Nat.eq_dec x n).
+    { subst. rewrite <- APP_EQ. reflexivity. }
+    { reflexivity. } }
+  { reflexivity. }
+  { simpl. rewrite IHt'1. rewrite IHt'2. reflexivity. }
 Qed.
 
-Lemma unify_most_general :
-  forall (t1 t2 : term) (m : subst),
-    unify t1 t2 (Some m) ->
-    forall (s : subst), unifier s t1 t2 -> more_general m s.
+Lemma mgu_most_general
+      (t1 t2 : term)
+      (m s : subst)
+      (UNI : mgu t1 t2 (Some m))
+      (S_UNIFIER : unifier s t1 t2) :
+      more_general m s.
 Proof.
-  intros t1 t2 m H. remember (Some m) as r eqn:eq.
-  generalize dependent eq. revert m.
-  induction H; intros m eq; inversion eq; clear eq.
-  * intros. unfold more_general. exists s. intros.
-    rewrite apply_empty. reflexivity.
-  * subst. specialize (IHunify r eq_refl).
+  revert S_UNIFIER. revert s.
+  remember (Some m) as r eqn:eq.
+  revert eq. revert m.
+  induction UNI; intros m eq; good_inversion eq.
+  { intros. unfold more_general. exists s. intros.
+    rewrite apply_empty. reflexivity. }
+  { subst. specialize (IHUNI r eq_refl).
     rename s into st. intros.
-    specialize (unification_step_binds_2 t1 t2 n st s e H0). intro.
-    assert (more_general r s).
-    { apply IHunify. unfold unifier. rewrite <- H1. rewrite <- H1. apply H0. }
-    unfold more_general in H2. destruct H2 as [d H2]. unfold more_general.
-    exists d. intro. rewrite compose_correctness. rewrite <- H2. apply H1.
+    specialize (unification_step_binds_2 _ _ _ _ _ STEP_SUBST S_UNIFIER). intro APP_EQ.
+    assert (MG : more_general r s).
+    { apply IHUNI. unfold unifier. congruence. }
+    unfold more_general in MG. destruct MG as [d MG]. unfold more_general.
+    exists d. intro. rewrite compose_correctness. congruence. }
 Qed.
 
-Lemma occurs_subst_height: forall s n t,
-  occurs n t = true -> height (apply_subst s (Var n)) <= height (apply_subst s t).
+Lemma occurs_subst_height
+      (s : subst)
+      (n : name)
+      (t : term)
+      (OCC : occurs n t = true) :
+      height (apply_subst s (Var n)) <= height (apply_subst s t).
 Proof.
-  intros. induction t.
-  * simpl in H. apply Nat.eqb_eq in H. subst. reflexivity.
-  * inversion H.
-  * simpl in H. apply Bool.orb_true_elim in H. destruct H.
-    + apply IHt1 in e. simpl. apply le_S. eapply le_trans.
-      eassumption. apply Nat.le_max_l.
-    + apply IHt2 in e. simpl. apply le_S. eapply le_trans.
-      eassumption. apply Nat.le_max_r.
+  induction t.
+  { simpl in OCC. apply Nat.eqb_eq in OCC. subst. reflexivity. }
+  { inversion OCC. }
+  { simpl in OCC. apply Bool.orb_true_elim in OCC. destruct OCC.
+    { apply IHt1 in e. simpl. apply le_S. eapply le_trans.
+      eassumption. apply Nat.le_max_l. }
+    { apply IHt2 in e. simpl. apply le_S. eapply le_trans.
+      eassumption. apply Nat.le_max_r. } }
 Qed.
 
-Lemma occurs_check_ground :
-  forall x t s,
-    occurs x t = true ->
-    apply_subst s (Var x) = apply_subst s t ->
-    Var x = t.
+Lemma occurs_check_ground
+      (s : subst)
+      (x : name)
+      (t : term)
+      (OCC : occurs x t = true)
+      (APP_EQ : apply_subst s (Var x) = apply_subst s t) :
+      Var x = t.
 Proof.
-  intros x t. destruct t.
-  * intros. simpl in H. apply beq_nat_true_iff in H. congruence.
-  * intros. inversion H.
-  * intros. exfalso. simpl in H. apply Bool.orb_true_elim in H. destruct H.
-    + apply occurs_subst_height with (s := s) in e. rewrite H0 in e.
+  destruct t.
+  { simpl in OCC. apply beq_nat_true_iff in OCC. congruence. }
+  { inversion OCC. }
+  { exfalso. simpl in OCC. apply Bool.orb_true_elim in OCC. destruct OCC.
+    { apply occurs_subst_height with (s := s) in e. rewrite APP_EQ in e.
       simpl in e. apply le_lt_n_Sm in e. apply lt_S_n in e.
       apply lt_irrefl with (height (apply_subst s t1)).
       eapply le_lt_trans.
       2: { eapply e. }
-      apply Nat.le_max_l.
-    + apply occurs_subst_height with (s := s) in e. rewrite H0 in e.
+      apply Nat.le_max_l. }
+    { apply occurs_subst_height with (s := s) in e. rewrite APP_EQ in e.
       simpl in e. apply le_lt_n_Sm in e. apply lt_S_n in e.
       apply lt_irrefl with (height (apply_subst s t2)).
       eapply le_lt_trans.
       2: { eapply e. }
-      apply Nat.le_max_r.
+      apply Nat.le_max_r. } }
 Qed.
 
-Lemma unify_non_unifiable :
-  forall (t1 t2 : term),
-    unify t1 t2 None -> forall s,  ~ (unifier s t1 t2).
+Lemma mgu_non_unifiable
+      (t1 t2 : term)
+      (UNI : mgu t1 t2 None)
+      (s : subst) :
+      ~ (unifier s t1 t2).
 Proof.
-  intros t1 t2 H. remember None as r eqn:eq.
-  induction H; inversion eq; clear eq.
-  * generalize dependent e. revert t2.
+  revert s. remember None as r eqn:eq.
+  induction UNI; good_inversion eq.
+  { revert STEP_NU. revert t2.
     induction t1; induction t2; intros H s; inversion H.
-    + destruct (Nat.eq_dec n n0).
-      - inversion H1.
-      - unfold create in H1. destruct (occurs n (Var n0)) eqn:eq; inversion H1.
-        intro C. specialize (occurs_check_ground n (Var n0) s eq C). intro.
-        inversion H0. contradiction.
-    + unfold create in H1. destruct (occurs n (Con n0 t2_1 t2_2)) eqn:eq; inversion H1.
-      intro C. specialize (occurs_check_ground n (Con n0 t2_1 t2_2) s eq C). intro.
-      inversion H0.
-    + destruct (Nat.eq_dec n n0).
-      - inversion H1.
-      - intro C. inversion C. contradiction.
-    + intro C. inversion C.
-    + unfold create in H1. destruct (occurs n0 (Con n t1_1 t1_2)) eqn:eq; inversion H1.
+    { destruct (Nat.eq_dec n n0).
+      { inversion H1. }
+      { unfold create in H1. destruct (occurs n (Var n0)) eqn:eq; inversion H1.
+        intro C. specialize (occurs_check_ground _ _ _ eq C). intro.
+        inversion H0. contradiction. } }
+    { unfold create in H1. destruct (occurs n (Con n0 t2_1 t2_2)) eqn:eq; inversion H1.
+      intro C. specialize (occurs_check_ground _ _ _ eq C). intro.
+      inversion H0. }
+    { destruct (Nat.eq_dec n n0).
+      { inversion H1. }
+      { intro C. inversion C. contradiction. } }
+    { intro C. inversion C. }
+    { unfold create in H1. destruct (occurs n0 (Con n t1_1 t1_2)) eqn:eq; inversion H1.
       intro C. red in C. symmetry in C.
-      specialize (occurs_check_ground n0 (Con n t1_1 t1_2) s eq C).
-      intro. inversion H0.
-    + intro C. inversion C.
-    + clear IHt2_1 IHt2_2. intro C. inversion C. destruct (Nat.eq_dec n n0).
-      - subst. destruct (unification_step t1_1 t2_1) eqn:eq.
+      specialize (occurs_check_ground _ _ _ eq C).
+      intro. inversion H0. }
+    { intro C. inversion C. }
+    { clear IHt2_1 IHt2_2. intro C. inversion C. destruct (Nat.eq_dec n n0).
+      { subst. destruct (unification_step t1_1 t2_1) eqn:eq.
         { eapply IHt1_1; eassumption. }
         { eapply IHt1_2; eassumption. }
-        { inversion H1. }
-      - contradiction.
-  * rename s into st. intros s C.
-    specialize (IHunify eq_refl s).
-    specialize (unification_step_binds_2 t1 t2 n st s e C). intros eq.
-    apply IHunify. red. rewrite <- eq. rewrite <- eq. assumption.
+        { inversion H1. } }
+      { contradiction. } } }
+  { rename s into st. intros s C.
+    specialize (IHUNI eq_refl s).
+    specialize (unification_step_binds_2 _ _ _ _ _ STEP_SUBST C). intros eq.
+    apply IHUNI. red. rewrite <- eq. rewrite <- eq. assumption. }
 Qed.
 
-Lemma MGU_dom
+Lemma mgu_dom
       (t1 t2 : term)
       (s : subst)
-      (MGU : unify t1 t2 (Some s))
+      (MGU : mgu t1 t2 (Some s))
       (x : name)
       (inDom : in_subst_dom s x) :
       In x (fv_term t1) \/ In x (fv_term t2).
-Proof. 
+Proof.
   remember (Some s) as r eqn:eq. revert eq inDom. revert s.
   induction MGU; intros; good_inversion eq.
   { destruct inDom. inversion H. }
@@ -746,10 +817,10 @@ Proof.
            eapply unification_step_fv; eauto. } } } }
 Qed.
 
-Lemma MGU_vran
+Lemma mgu_vran
       (t1 t2 : term)
       (s : subst)
-      (MGU : unify t1 t2 (Some s))
+      (MGU : mgu t1 t2 (Some s))
       (x : name)
       (inVRan : in_subst_vran s x) :
       In x (fv_term t1) \/ In x (fv_term t2).
