src/OpSemCompleteness.v
@@ -1,3 +1,5 @@
+Add LoadPath "~/JB/minikanren-coq/src/".
+
 Require Import List.
 Require Import Coq.Lists.ListSet.
 Import ListNotations.
@@ -11,33 +13,36 @@ Require Import Omega.
 Definition in_denotational_sem_subst (s : subst) (f : gt_fun) : Prop :=
   exists (f' : gt_fun), gt_fun_eq (subst_gt_fun_compose s f') f.
 
+Definition in_denotational_analog (t : trace) (f : gt_fun) : Prop :=
+  exists (s : subst) (n : nat), in_stream (Answer s n) t /\ in_denotational_sem_subst s f.
+
 Lemma set_empty_union
       (s1 s2 : var_set)
-      (eq : var_set_union s1 s2 = var_set_empty) :
+      (EQ : var_set_union s1 s2 = var_set_empty) :
       s1 = var_set_empty /\ s2 = var_set_empty.
 Proof.
   split.
   { destruct s1; auto.
     assert (In n var_set_empty).
-    { rewrite <- eq. apply set_union_intro. left. constructor. auto. }
+    { rewrite <- EQ. apply set_union_intro. left. constructor. auto. }
     inversion H. }
   { destruct s2; auto.
     assert (In n var_set_empty).
-    { rewrite <- eq. apply set_union_intro. right. constructor. auto. }
+    { rewrite <- EQ. apply set_union_intro. right. constructor. auto. }
     inversion H. }
 Qed.
 
 Lemma unfier_from_gt_unifier
       (t1 t2 : term)
       (f : gt_fun)
-      (f_unifies : gt_eq (apply_gt_fun f t1) (apply_gt_fun f t2)) :
+      (F_UNIFIES : gt_eq (apply_gt_fun f t1) (apply_gt_fun f t2)) :
       exists s, unifier s t1 t2 /\ in_denotational_sem_subst s f.
 Proof.
   remember (map (fun x => (x, proj1_sig (f x))) (var_set_union (fv_term t1) (fv_term t2))) as s.
   exists s. split.
-  { red. red in f_unifies.
+  { red. red in F_UNIFIES.
     assert (apply_subst s t1 = proj1_sig (apply_gt_fun f t1)).
-    { clear f_unifies.
+    { clear F_UNIFIES.
       assert (forall x, In x (fv_term t1) -> image s x = Some (proj1_sig (f x))).
       { intros. assert (In x (var_set_union (fv_term t1) (fv_term t2))).
         { apply set_union_intro1. auto. }
@@ -45,7 +50,7 @@ Proof.
         subst. apply map_image. auto. }
       apply subst_of_gt. auto. }
     assert (apply_subst s t2 = proj1_sig (apply_gt_fun f t2)).
-    { clear f_unifies.
+    { clear F_UNIFIES.
       assert (forall x, In x (fv_term t2) -> image s x = Some (proj1_sig (f x))).
       { intros. assert (In x (var_set_union (fv_term t1) (fv_term t2))).
         { apply set_union_intro2. auto. }
@@ -77,114 +82,165 @@ Proof.
     { red. auto. } }
 Qed.
 
-Inductive in_denotational_sem_state' : state' -> gt_fun -> Prop :=
-| dsst'Leaf : forall g s n f (Hgoal : in_denotational_sem_goal g f)
-                             (Hsubst : in_denotational_sem_subst s f),
-                             in_denotational_sem_state' (Leaf g s n) f
-| dsst'SumL : forall st1' st2' f (Hst1' : in_denotational_sem_state' st1' f),
-                                 in_denotational_sem_state' (Sum st1' st2') f
-| dsst'SumR : forall st1' st2' f (Hst2' : in_denotational_sem_state' st2' f),
-                                 in_denotational_sem_state' (Sum st1' st2') f
-| dsst'Prod : forall st' g f (Hgoal : in_denotational_sem_goal g f)
-                             (Hst' : in_denotational_sem_state' st' f),
-                             in_denotational_sem_state' (Prod st' g) f.
-
-Hint Constructors in_denotational_sem_state'.
-
-Inductive in_denotational_sem_state : state -> gt_fun -> Prop :=
-| dsstState : forall st' f (Hst' : in_denotational_sem_state' st' f),
-                           in_denotational_sem_state (State st') f.
-
-Hint Constructors in_denotational_sem_state.
-
-Definition in_denotational_analog (t : trace) (f : gt_fun) : Prop :=
-  exists (s : subst) (n : nat), in_stream (Answer s n) t /\ in_denotational_sem_subst s f.
-
-Lemma answer_correct
-      (s : subst)
-      (n : nat)
-      (f : gt_fun)
-      (HInDS : in_denotational_sem_subst s f)
-      (st' : state')
-      (st : state)
-      (EV : eval_step st' (Answer s n) st) :
-      in_denotational_sem_state' st' f.
+Lemma search_completeness_generalized
+      (l     : nat)
+      (g     : goal)
+      (CG    : consistent_goal g)
+      (s     : subst)
+      (n     : nat)
+      (WF : well_formed_state' (Leaf g s n))
+      (t     : trace)
+      (OP   : op_sem (State (Leaf g s n)) t)
+      (f     : gt_fun)
+      (DSG : in_denotational_sem_lev_goal l g f)
+      (DSS : in_denotational_sem_subst s f) :
+      exists (f' : gt_fun), (in_denotational_analog t f') /\
+                            forall (x : name), x < n -> gt_eq (f x) (f' x).
 Proof.
-  remember (Answer s n) as l.
-  induction EV; good_inversion Heql.
-  2, 3: auto.
-  destruct HInDS as [f' ff'_con].
-  constructor.
-  { constructor. red.
-    specialize (gt_fun_eq_apply _ _ t1 ff'_con). intro. rewrite <- H.
-    specialize (gt_fun_eq_apply _ _ t2 ff'_con). intro. rewrite <- H0.
-    rewrite gt_fun_apply_compose. rewrite gt_fun_apply_compose.
-    rewrite compose_correctness. rewrite compose_correctness.
-    apply unify_unifies in u. rewrite u. reflexivity. }
-  { red. exists (subst_gt_fun_compose s' f').
-    red. intros. red.
-    red in ff'_con. specialize (ff'_con x). red in ff'_con.
-    rewrite <- ff'_con. unfold subst_gt_fun_compose.
-    replace (fun x0 : name => apply_gt_fun f' (apply_subst s' (Var x0)))
-      with (subst_gt_fun_compose s' f').
-    2: reflexivity.
-    rewrite gt_fun_apply_compose. rewrite compose_correctness.
-    reflexivity. }
-Qed.
-
-Lemma next_state_correct
-      (f : gt_fun)
-      (st : state)
-      (HInDS : in_denotational_sem_state st f)
-      (st' : state')
-      (wfState : well_formed_state' st')
-      (h : label)
-      (EV : eval_step st' h st) :
-      in_denotational_sem_state' st' f.
-Proof.
-  induction EV; good_inversion HInDS.
-  { good_inversion Hst'.
-    { good_inversion Hst1'; constructor; auto. }
-    { good_inversion Hst2'; constructor; auto. } }
-  { good_inversion Hst'. good_inversion Hst'0. auto. }
-  { good_inversion wfState. good_inversion Hst'.
-    constructor; auto. econstructor; eauto.
-    intros HIn. apply FVLTCounter in HIn.
-    { omega. }
-    { reflexivity. } }
-  { good_inversion Hst'. auto. }
-  { auto. }
-  { good_inversion wfState. good_inversion Hst'; auto. }
-  { good_inversion Hst'. constructor; auto.
-    eapply answer_correct; eauto. }
-  { good_inversion wfState. good_inversion Hst'. auto. }
-  { good_inversion wfState. good_inversion Hst'.
-    { good_inversion Hst1'. constructor; auto.
-      eapply answer_correct; eauto. }
-    { good_inversion Hst2'. auto. } }
-Qed.
-
-Lemma search_correctness_generalized
-      (st   : state)
-      (wfSt : well_formed_state st)
-      (f    : gt_fun)
-      (t    : trace)
-      (HOP  : op_sem st t)
-      (HDA  : in_denotational_analog t f) :
-      in_denotational_sem_state st f.
-Proof.
-  revert HOP wfSt. revert st.
-  red in HDA. destruct HDA as [s [n [HInStr HInDS]]].
-  remember (Answer s n) as l. induction HInStr.
-  { intros. inversion HOP; clear HOP; subst.
-    constructor. eapply answer_correct; eauto. }
-  { specialize (IHHInStr Heql). intros.
-    inversion HOP; clear HOP; subst.
-    inversion wfSt; clear wfSt; subst.
-    specialize (well_formedness_preservation _ _ _ EV wfState).
-    intro wf_st0.
-    specialize (IHHInStr st0 OP wf_st0).
-    constructor. eapply next_state_correct; eauto. }
+  revert OP. revert t. revert CG DSG DSS WF. revert g f s n. induction l.
+  { intros. apply in_denotational_sem_zero_lev in DSG. contradiction. }
+  { induction g; intros; good_inversion CG.
+    { good_inversion DSG. }
+    { exists f. split.
+      { econstructor; eexists; split; eauto.
+        good_inversion OP. good_inversion EV. constructor. }
+      { intros; red; auto. } }
+    { exists f. split.
+      2: intros; red; auto.
+      good_inversion DSG. red in DSS. destruct DSS as [fs s_fs_f].
+      assert (gt_eq (apply_gt_fun fs (apply_subst s t)) (apply_gt_fun fs (apply_subst s t0))).
+      { red. rewrite <- gt_fun_apply_compose. rewrite <- gt_fun_apply_compose.
+        apply eq_trans with (proj1_sig (apply_gt_fun f t)).
+        { apply gt_fun_eq_apply. auto. }
+        { apply eq_trans with (proj1_sig (apply_gt_fun f t0)); auto.
+          symmetry. apply gt_fun_eq_apply. auto. } }
+      apply unfier_from_gt_unifier in H. destruct H as [u [u_uni u_fs]].
+      good_inversion OP. good_inversion EV.
+      { specialize (mgu_non_unifiable _ _ MGU u u_uni). contradiction. }
+      { rename s' into m. red. exists (compose s m). exists n. split; try constructor.
+        specialize (mgu_most_general _ _ _ u MGU u_uni). intro Hmg.
+        red in Hmg. destruct Hmg as [ds u_ds_m]. red in u_fs.
+        destruct u_fs as [fss u_fss_fs]. red. exists (subst_gt_fun_compose ds fss).
+        eapply gt_fun_eq_trans. 2: eauto.
+        eapply gt_fun_eq_trans. eapply subst_gt_fun_compose_assoc_subst.
+        eapply gt_fun_eq_trans. 2: eapply gt_fun_eq_compose; eauto.
+        apply gt_fun_eq_compose.
+        eapply gt_fun_eq_trans. red; symmetry; eapply subst_gt_fun_compose_assoc_subst.
+        apply gt_fun_compose_eq. intros. rewrite u_ds_m. apply compose_correctness. } }
+    { good_inversion OP. inversion EV; subst.
+      apply well_formedness_preservation in EV; auto. good_inversion EV.
+      good_inversion wfState.
+      specialize (op_sem_exists (State (Leaf g1 s n))). intro p1. destruct p1 as [t1 OP1].
+      specialize (op_sem_exists (State (Leaf g2 s n))). intro p2. destruct p2 as [t2 OP2].
+      specialize (sum_op_sem _ _ _ _ _ OP1 OP2 OP0). intro Hinter.
+      good_inversion DSG.
+      { specialize (IHg1 f s n CG_G1 DSG0 DSS WF_L t1 OP1).
+        destruct IHg1 as [f' [HinDA ff'_eq]]. exists f'. split; auto.
+        red in HinDA. destruct HinDA as [sr [nr [Hin DSSr]]].
+        red. exists sr. exists nr. split; auto. constructor.
+        apply (interleave_in _ _ _ Hinter (Answer sr nr)). auto. }
+      { specialize (IHg2 f s n CG_G2 DSG0 DSS WF_R t2 OP2).
+        destruct IHg2 as [f' [HinDA ff'_eq]]. exists f'. split; auto.
+        red in HinDA. destruct HinDA as [sr [nr [Hin DSSr]]].
+        red. exists sr. exists nr. split; auto. constructor.
+        apply (interleave_in _ _ _ Hinter (Answer sr nr)). auto. } }
+    { good_inversion DSG. good_inversion OP. inversion EV; subst.
+      specialize (op_sem_exists (State (Leaf g1 s n))). intro p1. destruct p1 as [t1 OP1].
+      assert (wfst'1 : well_formed_state' (Leaf g1 s n)).
+      { constructor; good_inversion WF; auto. }
+      specialize (IHg1 f s n CG_G1 DSG_L DSS wfst'1 t1 OP1).
+      destruct IHg1 as [f' [HinDA ff'_eq]]. red in HinDA.
+      destruct HinDA as [s' [n' [Hinstr' HDAS']]].
+      specialize (op_sem_exists (State (Leaf g2 s' n'))). intro p2. destruct p2 as [t2 OP2].
+      specialize (counter_in_trace _ _ _ _ _ _ OP1 Hinstr'). intro n_le_n'.
+      assert (wfst'2 : well_formed_state' (Leaf g2 s' n')).
+      { good_inversion WF.
+        specialize (well_formed_subst_in_trace _ (wfNonEmpty _ wfst'1)  _ OP1 _ _ Hinstr').
+        intros. destruct H.
+        constructor; auto. intros.
+        apply lt_le_trans with n; auto. }
+      assert (Hg2' : in_denotational_sem_lev_goal (S l) g2 f').
+      { apply den_sem_fv_only with f; auto. intros. apply ff'_eq.
+        good_inversion WF. auto. }
+      specialize (IHg2 f' s' n' CG_G2 Hg2' HDAS' wfst'2 t2 OP2).
+      destruct IHg2 as [f'' [HinDA f'f''_eq]]. red in HinDA.
+      destruct HinDA as [s'' [n'' [Hinstr'' HDAS'']]].
+      exists f''. split.
+      { red. exists s''. exists n''. split; auto.
+        constructor. eapply prod_op_sem_in; eauto. }
+      { intros. red. apply eq_trans with (proj1_sig (f' x)).
+        { apply ff'_eq. auto. }
+        { apply f'f''_eq. omega. } } }
+    { good_inversion DSG. good_inversion OP. inversion EV; subst.
+      apply well_formedness_preservation in EV; auto. good_inversion EV.
+      rename fn into fa.
+      red in DSS. destruct DSS as [fs fssf'_eq].
+      remember (fun x => if name_eq_dec x n
+                         then fa a
+                         else fs x) as fs'.
+      remember (fun x => if name_eq_dec x n
+                         then fa a
+                         else if name_eq_dec x a
+                              then (subst_gt_fun_compose s fs') a
+                              else fa x) as fn.
+      assert (H_n_is_fresh : forall x, In n (fv_term (apply_subst s (Var x))) -> x = n).
+      { intros. simpl in H0.
+        destruct (image s x) eqn:eq.
+        { assert (n < n).
+          { good_inversion WF. apply VRAN_LT_COUNTER.
+            red. eauto. }
+          omega. }
+        { simpl in H0. destruct H0; try contradiction. auto. } }
+      assert (Hgn : in_denotational_sem_lev_goal (S l) (g n) fn).
+      { rewrite Heqfn. good_inversion WF.
+        apply den_sem_another_fresh_var with n a fa; auto.
+        { intro C. apply FV_LT_COUNTER in C. omega. }
+        { destruct (name_eq_dec n n); try contradiction. reflexivity. }
+        { intros. destruct (name_eq_dec x n); try contradiction.
+          destruct (name_eq_dec x a); try contradiction. reflexivity. } }
+      assert (DSSn: in_denotational_sem_subst s fn).
+      { red. exists fs'. red. intros. red. unfold subst_gt_fun_compose.
+        rewrite Heqfs'. rewrite Heqfn. destruct (name_eq_dec x n).
+        { assert (H_n_is_fresh_2 : apply_subst s (Var n) = Var n).
+          { simpl. destruct (image s n) eqn:eq; auto.
+            good_inversion WF. assert (n < n).
+            { apply DOM_LT_COUNTER. red. eauto. }
+            omega. }
+          rewrite e. rewrite H_n_is_fresh_2. simpl.
+          destruct (name_eq_dec n n); try contradiction. auto. }
+        { destruct (name_eq_dec x a).
+          { rewrite e. rewrite Heqfs'. auto. }
+          { specialize (EASE x n1). rewrite EASE.
+            red in fssf'_eq. specialize (fssf'_eq x). red in fssf'_eq.
+            rewrite <- fssf'_eq. unfold subst_gt_fun_compose.
+            apply apply_gt_fun_fv. intros. destruct (name_eq_dec x0 n).
+            { rewrite e in H0. apply H_n_is_fresh in H0. contradiction. }
+            { reflexivity. } } } }
+      specialize (H n fn s (S n) (CG_BODY n) Hgn DSSn wfState t0 OP0).
+      destruct H as [f' [HinDA ff'_eq]]. exists f'. split.
+      { red. red in HinDA. destruct HinDA as [s' [n' [Hinstr HDAS]]].
+        exists s'. exists n'. split; auto. constructor; auto. }
+      { intros. assert (x < S n). { omega. }
+        specialize (ff'_eq x H0). red in ff'_eq. red. rewrite <- ff'_eq.
+        rewrite Heqfn. destruct (name_eq_dec x n); try omega.
+        destruct (name_eq_dec x a).
+        { rewrite e.
+          red in fssf'_eq. specialize (fssf'_eq a). red in fssf'_eq.
+          rewrite <- fssf'_eq. unfold subst_gt_fun_compose.
+          apply apply_gt_fun_fv. intros. rewrite Heqfs'.
+          destruct (name_eq_dec x0 n).
+          { auto. rewrite e0 in H1. apply H_n_is_fresh in H1. subst. contradiction. }
+          { unfold gt_eq. auto. } }
+        { specialize (EASE x n1). rewrite EASE. auto. } } }
+    { good_inversion DSG. good_inversion OP. inversion EV; subst.
+      apply well_formedness_preservation in EV; auto. good_inversion EV.
+      assert (cg_body : consistent_goal (proj1_sig (MiniKanrenSyntax.P n) t)).
+      { remember (MiniKanrenSyntax.P n) as d. destruct d as [rel [Hcl Hco]].
+        red in Hco. destruct (Hco t) as [Hcog Hcof]. auto. }
+      specialize (IHl (proj1_sig (MiniKanrenSyntax.P n) t) f s n0 cg_body DSG0 DSS wfState t1 OP0).
+      destruct IHl as [f' [HinDA ff'_eq]]. exists f'. split; auto.
+      red. red in HinDA. destruct HinDA as [s' [n' [Hinstr HDAS]]].
+      exists s'. exists n'. split; auto. constructor; auto. } }
 Qed.
 
 Fixpoint first_nats (k : nat) : list nat :=
@@ -200,205 +256,28 @@ Proof.
   { inversion H. { omega. } { apply IHk in H0. omega. } }
 Qed.
 
-Lemma search_correctness
-      (g   : goal)
-      (k   : nat)
-      (HC  : closed_goal_in_context (first_nats k) g)
-      (f   : gt_fun)
-      (t   : trace)
-      (HOP : op_sem (State (Leaf g empty_subst k)) t)
-      (HDA : in_denotational_analog t f) : in_denotational_sem_goal g f.
-Proof.
-  remember (State (Leaf g empty_subst k)) as st.
-  assert (in_denotational_sem_state st f).
-  { eapply search_correctness_generalized; eauto.
-    subst. constructor. constructor.
-    { intros. good_inversion H. good_inversion H0. }
-    { intros. good_inversion H. destruct H0 as [t1 [H1 _]]. good_inversion H1. }
-    { intros. apply HC in H. apply first_nats_less. auto. } }
-  subst. inversion H. inversion Hst'. auto.
-Qed.
-
-Lemma search_completeness_generalized
-      (l     : nat)
-      (g     : goal)
-      (Hcg    : consistent_goal g)
-      (s     : subst)
-      (n     : nat)
-      (wfSt' : well_formed_state' (Leaf g s n))
-      (t     : trace)
-      (HOP   : op_sem (State (Leaf g s n)) t)
-      (f     : gt_fun)
-      (Hgoal : in_denotational_sem_lev_goal l g f)
-      (Hsubst : in_denotational_sem_subst s f) :
-      exists (f' : gt_fun), (in_denotational_analog t f') /\
-                            forall (x : name), x < n -> gt_eq (f x) (f' x).
-Proof.
-  revert HOP. revert t. revert Hcg Hgoal Hsubst wfSt'. revert g f s n. induction l.
-  { intros. apply in_denotational_sem_zero_lev in Hgoal. contradiction. }
-  { induction g; intros; good_inversion Hcg.
-    { good_inversion Hgoal. }
-    { exists f. split.
-      2: intros; red; auto.
-      good_inversion Hgoal. red in Hsubst. destruct Hsubst as [fs s_fs_f].
-      assert (gt_eq (apply_gt_fun fs (apply_subst s t)) (apply_gt_fun fs (apply_subst s t0))).
-      { red. rewrite <- gt_fun_apply_compose. rewrite <- gt_fun_apply_compose.
-        apply eq_trans with (proj1_sig (apply_gt_fun f t)).
-        { apply gt_fun_eq_apply. auto. }
-        { apply eq_trans with (proj1_sig (apply_gt_fun f t0)); auto.
-          symmetry. apply gt_fun_eq_apply. auto. } }
-      apply unfier_from_gt_unifier in H. destruct H as [u [u_uni u_fs]].
-      good_inversion HOP. good_inversion EV.
-      { specialize (unify_non_unifiable _ _ H5 u u_uni). contradiction. }
-      { rename s' into m. red. exists (compose s m). exists n. split; try constructor.
-        specialize (unify_most_general _ _ _ H5 u u_uni). intro Hmg.
-        red in Hmg. destruct Hmg as [ds u_ds_m]. red in u_fs.
-        destruct u_fs as [fss u_fss_fs]. red. exists (subst_gt_fun_compose ds fss).
-        eapply gt_fun_eq_trans. 2: eauto.
-        eapply gt_fun_eq_trans. eapply subst_gt_fun_compose_assoc_subst.
-        eapply gt_fun_eq_trans. 2: eapply gt_fun_eq_compose; eauto.
-        apply gt_fun_eq_compose.
-        eapply gt_fun_eq_trans. red; symmetry; eapply subst_gt_fun_compose_assoc_subst.
-        apply gt_fun_compose_eq. intros. rewrite u_ds_m. apply compose_correctness. } }
-    { good_inversion HOP. inversion EV; subst.
-      apply well_formedness_preservation in EV; auto. good_inversion EV.
-      good_inversion wfState.
-      specialize (op_sem_exists (State (Leaf g1 s n))). intro p1. destruct p1 as [t1 OP1].
-      specialize (op_sem_exists (State (Leaf g2 s n))). intro p2. destruct p2 as [t2 OP2].
-      specialize (sum_op_sem _ _ _ _ _ OP1 OP2 OP). intro Hinter.
-      good_inversion Hgoal.
-      { specialize (IHg1 f s n Hcg1 Hg Hsubst wfst'1 t1 OP1).
-        destruct IHg1 as [f' [HinDA ff'_eq]]. exists f'. split; auto.
-        red in HinDA. destruct HinDA as [sr [nr [Hin Hsubstr]]].
-        red. exists sr. exists nr. split; auto. constructor.
-        apply (interleave_in _ _ _ Hinter (Answer sr nr)). auto. }
-      { specialize (IHg2 f s n Hcg2 Hg Hsubst wfst'2 t2 OP2).
-        destruct IHg2 as [f' [HinDA ff'_eq]]. exists f'. split; auto.
-        red in HinDA. destruct HinDA as [sr [nr [Hin Hsubstr]]].
-        red. exists sr. exists nr. split; auto. constructor.
-        apply (interleave_in _ _ _ Hinter (Answer sr nr)). auto. } }
-    { good_inversion Hgoal. good_inversion HOP. inversion EV; subst.
-      specialize (op_sem_exists (State (Leaf g1 s n))). intro p1. destruct p1 as [t1 OP1].
-      assert (wfst'1 : well_formed_state' (Leaf g1 s n)).
-      { constructor; good_inversion wfSt'; auto. }
-      specialize (IHg1 f s n Hcg1 Hg1 Hsubst wfst'1 t1 OP1).
-      destruct IHg1 as [f' [HinDA ff'_eq]]. red in HinDA.
-      destruct HinDA as [s' [n' [Hinstr' HDAS']]].
-      specialize (op_sem_exists (State (Leaf g2 s' n'))). intro p2. destruct p2 as [t2 OP2].
-      specialize (counter_in_trace _ _ _ _ _ _ OP1 Hinstr'). intro n_le_n'.
-      assert (wfst'2 : well_formed_state' (Leaf g2 s' n')).
-      { good_inversion wfSt'.
-        specialize (well_formed_subst_in_trace _ (wfNonEmpty _ wfst'1)  _ OP1 _ _ Hinstr').
-        intros. destruct H.
-        constructor; auto. intros.
-        apply lt_le_trans with n; auto. }
-      assert (Hg2' : in_denotational_sem_lev_goal (S l) g2 f').
-      { apply den_sem_fv_only with f; auto. intros. apply ff'_eq.
-        good_inversion wfSt'. auto. }
-      specialize (IHg2 f' s' n' Hcg2 Hg2' HDAS' wfst'2 t2 OP2).
-      destruct IHg2 as [f'' [HinDA f'f''_eq]]. red in HinDA.
-      destruct HinDA as [s'' [n'' [Hinstr'' HDAS'']]].
-      exists f''. split.
-      { red. exists s''. exists n''. split; auto.
-        constructor. eapply prod_op_sem_in; eauto. }
-      { intros. red. apply eq_trans with (proj1_sig (f' x)).
-        { apply ff'_eq. auto. }
-        { apply f'f''_eq. omega. } } }
-    { good_inversion Hgoal. good_inversion HOP. inversion EV; subst.
-      apply well_formedness_preservation in EV; auto. good_inversion EV.
-      rename fn into fa.
-      red in Hsubst. destruct Hsubst as [fs fssf'_eq].
-      remember (fun x => if name_eq_dec x n
-                         then fa a
-                         else fs x) as fs'.
-      remember (fun x => if name_eq_dec x n
-                         then fa a
-                         else if name_eq_dec x a
-                              then (subst_gt_fun_compose s fs') a
-                              else fa x) as fn.
-      assert (H_n_is_fresh : forall x, In n (fv_term (apply_subst s (Var x))) -> x = n).
-      { intros. simpl in H0.
-        destruct (image s x) eqn:eq.
-        { assert (n < n).
-          { good_inversion wfSt'. apply vranLTCounter.
-            red. eauto. }
-          omega. }
-        { simpl in H0. destruct H0; try contradiction. auto. } }
-      assert (Hgn : in_denotational_sem_lev_goal (S l) (g n) fn).
-      { rewrite Heqfn. good_inversion wfSt'.
-        apply den_sem_another_fresh_var with n a fa; auto.
-        { intro C. apply FVLTCounter in C. omega. }
-        { destruct (name_eq_dec n n); try contradiction. reflexivity. }
-        { intros. destruct (name_eq_dec x n); try contradiction.
-          destruct (name_eq_dec x a); try contradiction. reflexivity. } }
-      assert (Hsubstn: in_denotational_sem_subst s fn).
-      { red. exists fs'. red. intros. red. unfold subst_gt_fun_compose.
-        rewrite Heqfs'. rewrite Heqfn. destruct (name_eq_dec x n).
-        { assert (H_n_is_fresh_2 : apply_subst s (Var n) = Var n).
-          { simpl. destruct (image s n) eqn:eq; auto.
-            good_inversion wfSt'. assert (n < n).
-            { apply domLTCounter. red. eauto. }
-            omega. }
-          rewrite e. rewrite H_n_is_fresh_2. simpl.
-          destruct (name_eq_dec n n); try contradiction. auto. }
-        { destruct (name_eq_dec x a).
-          { rewrite e. rewrite Heqfs'. auto. }
-          { specialize (Hease x n1). rewrite Hease.
-            red in fssf'_eq. specialize (fssf'_eq x). red in fssf'_eq.
-            rewrite <- fssf'_eq. unfold subst_gt_fun_compose.
-            apply apply_gt_fun_fv. intros. destruct (name_eq_dec x0 n).
-            { rewrite e in H0. apply H_n_is_fresh in H0. contradiction. }
-            { reflexivity. } } } }
-      specialize (H n fn s (S n) (HcgInner n) Hgn Hsubstn wfState t0 OP).
-      destruct H as [f' [HinDA ff'_eq]]. exists f'. split.
-      { red. red in HinDA. destruct HinDA as [s' [n' [Hinstr HDAS]]].
-        exists s'. exists n'. split; auto. constructor; auto. }
-      { intros. assert (x < S n). { omega. }
-        specialize (ff'_eq x H0). red in ff'_eq. red. rewrite <- ff'_eq.
-        rewrite Heqfn. destruct (name_eq_dec x n); try omega.
-        destruct (name_eq_dec x a).
-        { rewrite e.
-          red in fssf'_eq. specialize (fssf'_eq a). red in fssf'_eq.
-          rewrite <- fssf'_eq. unfold subst_gt_fun_compose.
-          apply apply_gt_fun_fv. intros. rewrite Heqfs'.
-          destruct (name_eq_dec x0 n).
-          { auto. rewrite e0 in H1. apply H_n_is_fresh in H1. subst. contradiction. }
-          { unfold gt_eq. auto. } }
-        { specialize (Hease x n1). rewrite Hease. auto. } } }
-    { good_inversion Hgoal. good_inversion HOP. inversion EV; subst.
-      apply well_formedness_preservation in EV; auto. good_inversion EV.
-      assert (cg_body : consistent_goal (proj1_sig (MiniKanrenSyntax.P n) t)).
-      { remember (MiniKanrenSyntax.P n) as d. destruct d as [rel [Hcl Hco]].
-        red in Hco. destruct (Hco t) as [Hcog Hcof]. auto. }
-      specialize (IHl (proj1_sig (MiniKanrenSyntax.P n) t) f s n0 cg_body Hbody Hsubst wfState t1 OP).
-      destruct IHl as [f' [HinDA ff'_eq]]. exists f'. split; auto.
-      red. red in HinDA. destruct HinDA as [s' [n' [Hinstr HDAS]]].
-      exists s'. exists n'. split; auto. constructor; auto. } }
-Qed.
-
-
 Lemma search_completeness
       (g   : goal)
-      (Hcg    : consistent_goal g)
+      (CG    : consistent_goal g)
       (k   : nat)
       (HC  : closed_goal_in_context (first_nats k) g)
       (f   : gt_fun)
       (t   : trace)
-      (HOP : op_sem (State (Leaf g empty_subst k)) t)
+      (OP : op_sem (State (Leaf g empty_subst k)) t)
       (HDS : in_denotational_sem_goal g f) :
       exists (f' : gt_fun), (in_denotational_analog t f') /\
                             forall (x : name), In x (first_nats k) -> gt_eq (f x) (f' x).
 Proof.
   apply in_denotational_sem_some_lev in HDS. destruct HDS as [l HDS].
-  assert (wfSt' : well_formed_state' (Leaf g empty_subst k)).
+  assert (WF : well_formed_state' (Leaf g empty_subst k)).
   { constructor.
-    { intros. good_inversion H. good_inversion H0. }
-    { intros. good_inversion H. destruct H0 as [t1 [H1 _]]. good_inversion H1. }
+    { intros. good_inversion X_IN_DOM. good_inversion H. }
+    { intros. good_inversion X_IN_VRAN. destruct H as [t0 [H0 _]]. good_inversion H0. }
     { red in HC. intros. apply first_nats_less; auto. } }
-  assert (Hsubst : in_denotational_sem_subst empty_subst f).
+  assert (DSS : in_denotational_sem_subst empty_subst f).
   { red. exists f. red. intros.
     unfold subst_gt_fun_compose. rewrite apply_empty. reflexivity. }
-  specialize (search_completeness_generalized l g Hcg empty_subst k wfSt' t HOP f HDS Hsubst).
+  specialize (search_completeness_generalized l g CG empty_subst k WF t OP f HDS DSS).
   intro. destruct H as [f' [HinDA ff'eq]]. exists f'. split; auto.
   intros. apply ff'eq. apply first_nats_less; auto.
 Qed.
